Move to bundled universes.

Structure/Generic/Axioms.lean
@@ -18,8 +18,9 @@ import Structure.Generic.Notation
 
 
 set_option autoBoundImplicitLocal false
+set_option pp.universes true
 
-universes u v w w'
+universes u uu v vv w
 
 
 
@@ -29,14 +30,58 @@ universes u v w w'
 -- * Another common case is `Bundled C` for a type class `C : Sort u → Sort v`.
 -- Both examples are defined in `Instances.lean`.
 
-class HasInstances (V : Sort v) where
-(Inst : V → Sort u)
+class HasInstances (U : Sort uu) where
+(Inst : U → Sort u)
 
 namespace HasInstances
 
   instance coeSort (V : Sort v) [s : HasInstances V] : CoeSort V (Sort u) := ⟨s.Inst⟩
 
+  notation "⌈" V:0 "⌉" => HasInstances.Inst V
+
+  instance sortHasInstances : HasInstances (Sort u) := ⟨id⟩
+
 end HasInstances
+
+
+
+def TypeClass (U : Sort uu) [HasInstances.{u, uu} U] := U → Sort v
+
+structure Bundled {U : Sort uu} [HasInstances.{u, uu} U] (C : TypeClass.{u, uu, v} U) : Sort (max 1 uu v) where
+(α    : U)
+[inst : C α]
+
+namespace Bundled
+
+  instance hasInstances {U : Sort uu} [HasInstances.{u, uu} U] (C : TypeClass.{u, uu, v} U) : HasInstances (Bundled C) :=
+  ⟨λ S => ⌈S.α⌉⟩
+
+end Bundled
+
+
+
+def Universe : Type (max u uu) := Bundled HasInstances.{u, uu}
+
+namespace Universe
+
+  instance hasInstances : HasInstances Universe.{u, uu} := Bundled.hasInstances HasInstances
+
+  variable (U : Universe)
+
+  instance instInst : HasInstances U.α := U.inst
+  instance : HasInstances ⌈U⌉ := instInst U
+
+end Universe
+
+def sortUniverse : Universe.{u, u + 1} := ⟨Sort u⟩
+@[reducible] def propUniverse := sortUniverse.{0}
+@[reducible] def typeUniverse := sortUniverse.{u + 1}
+
+def universeUniverse : Universe.{uu, (max u uu) + 1} := ⟨Universe.{u, uu}⟩
+
+
+
+-- TODO: What we want of `universeUniverse` is: It has functors, and such a functor is a more restricted type class.
 
 
 
@@ -62,136 +107,118 @@ end HasInstances
 --
 -- Moreover, `α ⟶' β` is defined so that `α` and `β` can live in different universes.
 
-class HasIsFun (V : Sort v) (W : Sort w) [HasInstances V] [HasInstances W] where
-(IsFun {α : V} {β : W} : (α → β) → Sort u)
+class HasExternalFunctors (U : Universe.{u, uu}) (V : Universe.{v, vv}) where
+(IsFun {α : U} {β : V} : (α → β) → Sort w)
 
-structure BundledFunctor {V : Sort v} {W : Sort w} [HasInstances V] [HasInstances W] [h : HasIsFun V W]
-                         (α : V) (β : W) where
+structure BundledFunctor {U V : Universe} [h : HasExternalFunctors.{u, uu, v, vv, w} U V] (α : U) (β : V) : Sort (max 1 u v w) where
 (f     : α → β)
 (isFun : h.IsFun f)
 
 namespace BundledFunctor
 
-  variable {V : Sort v} {W : Sort w} [HasInstances V] [HasInstances W] [h : HasIsFun V W]
+  variable {U V : Universe} [h : HasExternalFunctors U V]
 
   infixr:20 " ⟶' " => BundledFunctor
 
-  instance coeFun (α : V) (β : W) : CoeFun (α ⟶' β) (λ _ => α → β) := ⟨BundledFunctor.f⟩
+  instance coeFun (α : U) (β : V) : CoeFun (α ⟶' β) (λ _ => α → β) := ⟨BundledFunctor.f⟩
 
 end BundledFunctor
 
-class HasFun (V : Sort v) extends HasInstances V, HasIsFun V V where
-(Fun                : V → V → V)
-(funEquiv (α β : V) : Inst (Fun α β) ≃ (α ⟶' β))
+class HasInternalFunctors (U : Universe) extends HasExternalFunctors U U where
+(Fun                : U → U → U)
+(funEquiv (α β : U) : ⌈Fun α β⌉ ≃ (α ⟶' β))
 
-namespace HasFun
+namespace HasInternalFunctors
 
-  variable {V : Sort v} [h : HasFun V]
+  variable {U : Universe} [h : HasInternalFunctors U]
 
   -- This is potentially endless. Is there a better way?
-  instance hasArrow : HasArrow     V                             V              := ⟨h.Fun⟩
-  instance : HasFun   (            V             (⟶)             V            ) := h
-  instance : HasArrow              V                 (    V     (⟶)     V    )  := hasArrow
-  instance : HasFun   (            V             (⟶) (    V     (⟶)     V    )) := h
-  instance : HasArrow  (    V     (⟶)     V    )                 V              := hasArrow
-  instance : HasFun   ((    V     (⟶)     V    ) (⟶)             V            ) := h
-  instance : HasArrow  (    V     (⟶)     V    )     (    V     (⟶)     V    )  := hasArrow
-  instance : HasFun   ((    V     (⟶)     V    ) (⟶) (    V     (⟶)     V    )) := h
-  instance : HasArrow              V                 (    V     (⟶) (V (⟶) V))  := hasArrow
-  instance : HasFun   (            V             (⟶) (    V     (⟶) (V (⟶) V))) := h
-  instance : HasArrow  (    V     (⟶)     V    )     (    V     (⟶) (V (⟶) V))  := hasArrow
-  instance : HasFun   ((    V     (⟶)     V    ) (⟶) (    V     (⟶) (V (⟶) V))) := h
-  instance : HasArrow              V                 ((V (⟶) V) (⟶)     V    )  := hasArrow
-  instance : HasFun   (            V             (⟶) ((V (⟶) V) (⟶)     V    )) := h
-  instance : HasArrow              V                 ((V (⟶) V) (⟶) (V (⟶) V))  := hasArrow
-  instance : HasFun   (            V             (⟶) ((V (⟶) V) (⟶) (V (⟶) V))) := h
-  instance : HasArrow  (    V     (⟶)     V    )     ((V (⟶) V) (⟶)     V    )  := hasArrow
-  instance : HasFun   ((    V     (⟶)     V    ) (⟶) ((V (⟶) V) (⟶)     V    )) := h
-  instance : HasArrow  (    V     (⟶)     V    )     ((V (⟶) V) (⟶) (V (⟶) V))  := hasArrow
-  instance : HasFun   ((    V     (⟶)     V    ) (⟶) ((V (⟶) V) (⟶) (V (⟶) V))) := h
-  instance : HasArrow  (    V     (⟶) (V (⟶) V))                 V              := hasArrow
-  instance : HasFun   ((    V     (⟶) (V (⟶) V)) (⟶)             V            ) := h
-  instance : HasArrow  (    V     (⟶) (V (⟶) V))     (    V     (⟶)     V    )  := hasArrow
-  instance : HasFun   ((    V     (⟶) (V (⟶) V)) (⟶) (    V     (⟶)     V    )) := h
-  instance : HasArrow  (    V     (⟶) (V (⟶) V))     (    V     (⟶) (V (⟶) V))  := hasArrow
-  instance : HasFun   ((    V     (⟶) (V (⟶) V)) (⟶) (    V     (⟶) (V (⟶) V))) := h
-  instance : HasArrow  (    V     (⟶) (V (⟶) V))     ((V (⟶) V) (⟶)     V    )  := hasArrow
-  instance : HasFun   ((    V     (⟶) (V (⟶) V)) (⟶) ((V (⟶) V) (⟶)     V    )) := h
-  instance : HasArrow  (    V     (⟶) (V (⟶) V))     ((V (⟶) V) (⟶) (V (⟶) V))  := hasArrow
-  instance : HasFun   ((    V     (⟶) (V (⟶) V)) (⟶) ((V (⟶) V) (⟶) (V (⟶) V))) := h
-  instance : HasArrow  ((V (⟶) V) (⟶)     V    )                 V              := hasArrow
-  instance : HasFun   (((V (⟶) V) (⟶)     V    ) (⟶)             V            ) := h
-  instance : HasArrow  ((V (⟶) V) (⟶)     V    )     (    V     (⟶)     V    )  := hasArrow
-  instance : HasFun   (((V (⟶) V) (⟶)     V    ) (⟶) (    V     (⟶)     V    )) := h
-  instance : HasArrow  ((V (⟶) V) (⟶)     V    )     (    V     (⟶) (V (⟶) V))  := hasArrow
-  instance : HasFun   (((V (⟶) V) (⟶)     V    ) (⟶) (    V     (⟶) (V (⟶) V))) := h
-  instance : HasArrow  ((V (⟶) V) (⟶)     V    )     ((V (⟶) V) (⟶)     V    )  := hasArrow
-  instance : HasFun   (((V (⟶) V) (⟶)     V    ) (⟶) ((V (⟶) V) (⟶)     V    )) := h
-  instance : HasArrow  ((V (⟶) V) (⟶)     V    )     ((V (⟶) V) (⟶) (V (⟶) V))  := hasArrow
-  instance : HasFun   (((V (⟶) V) (⟶)     V    ) (⟶) ((V (⟶) V) (⟶) (V (⟶) V))) := h
-  instance : HasArrow  ((V (⟶) V) (⟶) (V (⟶) V))                 V              := hasArrow
-  instance : HasFun   (((V (⟶) V) (⟶) (V (⟶) V)) (⟶)             V            ) := h
-  instance : HasArrow  ((V (⟶) V) (⟶) (V (⟶) V))     (    V     (⟶)     V    )  := hasArrow
-  instance : HasFun   (((V (⟶) V) (⟶) (V (⟶) V)) (⟶) (    V     (⟶)     V    )) := h
-  instance : HasArrow  ((V (⟶) V) (⟶) (V (⟶) V))     (    V     (⟶) (V (⟶) V))  := hasArrow
-  instance : HasFun   (((V (⟶) V) (⟶) (V (⟶) V)) (⟶) (    V     (⟶) (V (⟶) V))) := h
-  instance : HasArrow  ((V (⟶) V) (⟶) (V (⟶) V))     ((V (⟶) V) (⟶)     V    )  := hasArrow
-  instance : HasFun   (((V (⟶) V) (⟶) (V (⟶) V)) (⟶) ((V (⟶) V) (⟶)     V    )) := h
-  instance : HasArrow  ((V (⟶) V) (⟶) (V (⟶) V))     ((V (⟶) V) (⟶) (V (⟶) V))  := hasArrow
-  instance : HasFun   (((V (⟶) V) (⟶) (V (⟶) V)) (⟶) ((V (⟶) V) (⟶) (V (⟶) V))) := h
+  instance hasArrow : HasArrow             ⌈U⌉                                   ⌈U⌉                 := ⟨h.Fun⟩
+  instance : HasInstances  (               ⌈U⌉                (⟶)                ⌈U⌉               ) := Universe.instInst U
+  instance : HasArrow                      ⌈U⌉                    (     ⌈U⌉      (⟶)      ⌈U⌉     )  := hasArrow
+  instance : HasInstances  (               ⌈U⌉                (⟶) (     ⌈U⌉      (⟶)      ⌈U⌉     )) := Universe.instInst U
+  instance : HasArrow       (     ⌈U⌉      (⟶)      ⌈U⌉     )                    ⌈U⌉                 := hasArrow
+  instance : HasInstances  ((     ⌈U⌉      (⟶)      ⌈U⌉     ) (⟶)                ⌈U⌉               ) := Universe.instInst U
+  instance : HasArrow       (     ⌈U⌉      (⟶)      ⌈U⌉     )     (     ⌈U⌉      (⟶)      ⌈U⌉     )  := hasArrow
+  instance : HasInstances  ((     ⌈U⌉      (⟶)      ⌈U⌉     ) (⟶) (     ⌈U⌉      (⟶)      ⌈U⌉     )) := Universe.instInst U
+  instance : HasArrow                      ⌈U⌉                    (     ⌈U⌉      (⟶) (⌈U⌉ (⟶) ⌈U⌉))  := hasArrow
+  instance : HasInstances  (               ⌈U⌉                (⟶) (     ⌈U⌉      (⟶) (⌈U⌉ (⟶) ⌈U⌉))) := Universe.instInst U
+  instance : HasArrow       (     ⌈U⌉      (⟶)      ⌈U⌉     )     (     ⌈U⌉      (⟶) (⌈U⌉ (⟶) ⌈U⌉))  := hasArrow
+  instance : HasInstances  ((     ⌈U⌉      (⟶)      ⌈U⌉     ) (⟶) (     ⌈U⌉      (⟶) (⌈U⌉ (⟶) ⌈U⌉))) := Universe.instInst U
+  instance : HasArrow                      ⌈U⌉                    ((⌈U⌉ (⟶) ⌈U⌉) (⟶)      ⌈U⌉     )  := hasArrow
+  instance : HasInstances  (               ⌈U⌉                (⟶) ((⌈U⌉ (⟶) ⌈U⌉) (⟶)      ⌈U⌉     )) := Universe.instInst U
+  instance : HasArrow                      ⌈U⌉                    ((⌈U⌉ (⟶) ⌈U⌉) (⟶) (⌈U⌉ (⟶) ⌈U⌉))  := hasArrow
+  instance : HasInstances  (               ⌈U⌉                (⟶) ((⌈U⌉ (⟶) ⌈U⌉) (⟶) (⌈U⌉ (⟶) ⌈U⌉))) := Universe.instInst U
+  instance : HasArrow       (     ⌈U⌉      (⟶)      ⌈U⌉     )     ((⌈U⌉ (⟶) ⌈U⌉) (⟶)      ⌈U⌉     )  := hasArrow
+  instance : HasInstances  ((     ⌈U⌉      (⟶)      ⌈U⌉     ) (⟶) ((⌈U⌉ (⟶) ⌈U⌉) (⟶)      ⌈U⌉     )) := Universe.instInst U
+  instance : HasArrow       (     ⌈U⌉      (⟶)      ⌈U⌉     )     ((⌈U⌉ (⟶) ⌈U⌉) (⟶) (⌈U⌉ (⟶) ⌈U⌉))  := hasArrow
+  instance : HasInstances  ((     ⌈U⌉      (⟶)      ⌈U⌉     ) (⟶) ((⌈U⌉ (⟶) ⌈U⌉) (⟶) (⌈U⌉ (⟶) ⌈U⌉))) := Universe.instInst U
+  instance : HasArrow       (     ⌈U⌉      (⟶) (⌈U⌉ (⟶) ⌈U⌉))                    ⌈U⌉                 := hasArrow
+  instance : HasInstances  ((     ⌈U⌉      (⟶) (⌈U⌉ (⟶) ⌈U⌉)) (⟶)                ⌈U⌉               ) := Universe.instInst U
+  instance : HasArrow       (     ⌈U⌉      (⟶) (⌈U⌉ (⟶) ⌈U⌉))     (     ⌈U⌉      (⟶)      ⌈U⌉     )  := hasArrow
+  instance : HasInstances  ((     ⌈U⌉      (⟶) (⌈U⌉ (⟶) ⌈U⌉)) (⟶) (     ⌈U⌉      (⟶)      ⌈U⌉     )) := Universe.instInst U
+  instance : HasArrow       (     ⌈U⌉      (⟶) (⌈U⌉ (⟶) ⌈U⌉))     (     ⌈U⌉      (⟶) (⌈U⌉ (⟶) ⌈U⌉))  := hasArrow
+  instance : HasInstances  ((     ⌈U⌉      (⟶) (⌈U⌉ (⟶) ⌈U⌉)) (⟶) (     ⌈U⌉      (⟶) (⌈U⌉ (⟶) ⌈U⌉))) := Universe.instInst U
+  instance : HasArrow       (     ⌈U⌉      (⟶) (⌈U⌉ (⟶) ⌈U⌉))     ((⌈U⌉ (⟶) ⌈U⌉) (⟶)      ⌈U⌉     )  := hasArrow
+  instance : HasInstances  ((     ⌈U⌉      (⟶) (⌈U⌉ (⟶) ⌈U⌉)) (⟶) ((⌈U⌉ (⟶) ⌈U⌉) (⟶)      ⌈U⌉     )) := Universe.instInst U
+  instance : HasArrow       (     ⌈U⌉      (⟶) (⌈U⌉ (⟶) ⌈U⌉))     ((⌈U⌉ (⟶) ⌈U⌉) (⟶) (⌈U⌉ (⟶) ⌈U⌉))  := hasArrow
+  instance : HasInstances  ((     ⌈U⌉      (⟶) (⌈U⌉ (⟶) ⌈U⌉)) (⟶) ((⌈U⌉ (⟶) ⌈U⌉) (⟶) (⌈U⌉ (⟶) ⌈U⌉))) := Universe.instInst U
+  instance : HasArrow       ((⌈U⌉ (⟶) ⌈U⌉) (⟶)      ⌈U⌉     )                    ⌈U⌉                 := hasArrow
+  instance : HasInstances  (((⌈U⌉ (⟶) ⌈U⌉) (⟶)      ⌈U⌉     ) (⟶)                ⌈U⌉               ) := Universe.instInst U
+  instance : HasArrow       ((⌈U⌉ (⟶) ⌈U⌉) (⟶)      ⌈U⌉     )     (     ⌈U⌉      (⟶)      ⌈U⌉     )  := hasArrow
+  instance : HasInstances  (((⌈U⌉ (⟶) ⌈U⌉) (⟶)      ⌈U⌉     ) (⟶) (     ⌈U⌉      (⟶)      ⌈U⌉     )) := Universe.instInst U
+  instance : HasArrow       ((⌈U⌉ (⟶) ⌈U⌉) (⟶)      ⌈U⌉     )     (     ⌈U⌉      (⟶) (⌈U⌉ (⟶) ⌈U⌉))  := hasArrow
+  instance : HasInstances  (((⌈U⌉ (⟶) ⌈U⌉) (⟶)      ⌈U⌉     ) (⟶) (     ⌈U⌉      (⟶) (⌈U⌉ (⟶) ⌈U⌉))) := Universe.instInst U
+  instance : HasArrow       ((⌈U⌉ (⟶) ⌈U⌉) (⟶)      ⌈U⌉     )     ((⌈U⌉ (⟶) ⌈U⌉) (⟶)      ⌈U⌉     )  := hasArrow
+  instance : HasInstances  (((⌈U⌉ (⟶) ⌈U⌉) (⟶)      ⌈U⌉     ) (⟶) ((⌈U⌉ (⟶) ⌈U⌉) (⟶)      ⌈U⌉     )) := Universe.instInst U
+  instance : HasArrow       ((⌈U⌉ (⟶) ⌈U⌉) (⟶)      ⌈U⌉     )     ((⌈U⌉ (⟶) ⌈U⌉) (⟶) (⌈U⌉ (⟶) ⌈U⌉))  := hasArrow
+  instance : HasInstances  (((⌈U⌉ (⟶) ⌈U⌉) (⟶)      ⌈U⌉     ) (⟶) ((⌈U⌉ (⟶) ⌈U⌉) (⟶) (⌈U⌉ (⟶) ⌈U⌉))) := Universe.instInst U
+  instance : HasArrow       ((⌈U⌉ (⟶) ⌈U⌉) (⟶) (⌈U⌉ (⟶) ⌈U⌉))                    ⌈U⌉                 := hasArrow
+  instance : HasInstances  (((⌈U⌉ (⟶) ⌈U⌉) (⟶) (⌈U⌉ (⟶) ⌈U⌉)) (⟶)                ⌈U⌉               ) := Universe.instInst U
+  instance : HasArrow       ((⌈U⌉ (⟶) ⌈U⌉) (⟶) (⌈U⌉ (⟶) ⌈U⌉))     (     ⌈U⌉      (⟶)      ⌈U⌉     )  := hasArrow
+  instance : HasInstances  (((⌈U⌉ (⟶) ⌈U⌉) (⟶) (⌈U⌉ (⟶) ⌈U⌉)) (⟶) (     ⌈U⌉      (⟶)      ⌈U⌉     )) := Universe.instInst U
+  instance : HasArrow       ((⌈U⌉ (⟶) ⌈U⌉) (⟶) (⌈U⌉ (⟶) ⌈U⌉))     (     ⌈U⌉      (⟶) (⌈U⌉ (⟶) ⌈U⌉))  := hasArrow
+  instance : HasInstances  (((⌈U⌉ (⟶) ⌈U⌉) (⟶) (⌈U⌉ (⟶) ⌈U⌉)) (⟶) (     ⌈U⌉      (⟶) (⌈U⌉ (⟶) ⌈U⌉))) := Universe.instInst U
+  instance : HasArrow       ((⌈U⌉ (⟶) ⌈U⌉) (⟶) (⌈U⌉ (⟶) ⌈U⌉))     ((⌈U⌉ (⟶) ⌈U⌉) (⟶)      ⌈U⌉     )  := hasArrow
+  instance : HasInstances  (((⌈U⌉ (⟶) ⌈U⌉) (⟶) (⌈U⌉ (⟶) ⌈U⌉)) (⟶) ((⌈U⌉ (⟶) ⌈U⌉) (⟶)      ⌈U⌉     )) := Universe.instInst U
+  instance : HasArrow       ((⌈U⌉ (⟶) ⌈U⌉) (⟶) (⌈U⌉ (⟶) ⌈U⌉))     ((⌈U⌉ (⟶) ⌈U⌉) (⟶) (⌈U⌉ (⟶) ⌈U⌉))  := hasArrow
+  instance : HasInstances  (((⌈U⌉ (⟶) ⌈U⌉) (⟶) (⌈U⌉ (⟶) ⌈U⌉)) (⟶) ((⌈U⌉ (⟶) ⌈U⌉) (⟶) (⌈U⌉ (⟶) ⌈U⌉))) := Universe.instInst U
 
-  instance : HasIsFun              V                 (    V     (⟶)     V    )  := h.toHasIsFun
-  instance : HasIsFun  (    V     (⟶)     V    )                 V              := h.toHasIsFun
-  instance : HasIsFun              V                 (    V     (⟶) (V (⟶) V))  := h.toHasIsFun
-  instance : HasIsFun  (    V     (⟶)     V    )     (    V     (⟶) (V (⟶) V))  := h.toHasIsFun
-  instance : HasIsFun              V                 ((V (⟶) V) (⟶)     V    )  := h.toHasIsFun
-  instance : HasIsFun              V                 ((V (⟶) V) (⟶) (V (⟶) V))  := h.toHasIsFun
-  instance : HasIsFun  (    V     (⟶)     V    )     ((V (⟶) V) (⟶)     V    )  := h.toHasIsFun
-  instance : HasIsFun  (    V     (⟶)     V    )     ((V (⟶) V) (⟶) (V (⟶) V))  := h.toHasIsFun
-  instance : HasIsFun  (    V     (⟶) (V (⟶) V))                 V              := h.toHasIsFun
-  instance : HasIsFun  (    V     (⟶) (V (⟶) V))     (    V     (⟶)     V    )  := h.toHasIsFun
-  instance : HasIsFun  (    V     (⟶) (V (⟶) V))     ((V (⟶) V) (⟶)     V    )  := h.toHasIsFun
-  instance : HasIsFun  (    V     (⟶) (V (⟶) V))     ((V (⟶) V) (⟶) (V (⟶) V))  := h.toHasIsFun
-  instance : HasIsFun  ((V (⟶) V) (⟶)     V    )                 V              := h.toHasIsFun
-  instance : HasIsFun  ((V (⟶) V) (⟶)     V    )     (    V     (⟶)     V    )  := h.toHasIsFun
-  instance : HasIsFun  ((V (⟶) V) (⟶)     V    )     (    V     (⟶) (V (⟶) V))  := h.toHasIsFun
-  instance : HasIsFun  ((V (⟶) V) (⟶)     V    )     ((V (⟶) V) (⟶) (V (⟶) V))  := h.toHasIsFun
-  instance : HasIsFun  ((V (⟶) V) (⟶) (V (⟶) V))                 V              := h.toHasIsFun
-  instance : HasIsFun  ((V (⟶) V) (⟶) (V (⟶) V))     (    V     (⟶)     V    )  := h.toHasIsFun
-  instance : HasIsFun  ((V (⟶) V) (⟶) (V (⟶) V))     (    V     (⟶) (V (⟶) V))  := h.toHasIsFun
-  instance : HasIsFun  ((V (⟶) V) (⟶) (V (⟶) V))     ((V (⟶) V) (⟶)     V    )  := h.toHasIsFun
+  def toBundled   {α β : U} (F : α ⟶  β) : α ⟶' β := (h.funEquiv α β).toFun  F
+  def fromBundled {α β : U} (F : α ⟶' β) : α ⟶  β := (h.funEquiv α β).invFun F
 
-  def toBundled   {α β : V} (F : α ⟶  β) : α ⟶' β := (h.funEquiv α β).toFun  F
-  def fromBundled {α β : V} (F : α ⟶' β) : α ⟶  β := (h.funEquiv α β).invFun F
+  @[simp] theorem fromToBundled {α β : U} (F : α ⟶  β) : fromBundled (toBundled F) = F := (h.funEquiv α β).leftInv  F
+  @[simp] theorem toFromBundled {α β : U} (F : α ⟶' β) : toBundled (fromBundled F) = F := (h.funEquiv α β).rightInv F
 
-  @[simp] theorem fromToBundled {α β : V} (F : α ⟶  β) : fromBundled (toBundled F) = F := (h.funEquiv α β).leftInv  F
-  @[simp] theorem toFromBundled {α β : V} (F : α ⟶' β) : toBundled (fromBundled F) = F := (h.funEquiv α β).rightInv F
+  def funCoe {α β : U} (F : α ⟶ β) : α → β := (toBundled F).f
+  instance coeFun (α β : U) : CoeFun ⌈α ⟶ β⌉ (λ _ => α → β) := ⟨funCoe⟩
 
-  def funCoe {α β : V} (F : α ⟶ β) : α → β := (toBundled F).f
-  instance coeFun (α β : V) : CoeFun (h.Inst (α ⟶ β)) (λ _ => α → β) := ⟨funCoe⟩
+  -- Workaround for cases where `coeFun` doesn't work.
+  notation:max F:max "⟮" x:0 "⟯" => HasInternalFunctors.funCoe F x
 
-  def isFun {α β : V} (F : α ⟶ β) : h.IsFun (funCoe F) := (toBundled F).isFun
+  def isFun {α β : U} (F : α ⟶ β) : h.IsFun (funCoe F) := (toBundled F).isFun
 
-  theorem toBundled.eff {α β : V} (F : α ⟶ β) (a : α) : (toBundled F) a = F a := rfl
+  theorem toBundled.eff {α β : U} (F : α ⟶ β) (a : α) : (toBundled F) a = F a := rfl
 
-  @[simp] theorem fromBundled.coe {α β : V} (F : α ⟶' β) : funCoe (fromBundled F) = F.f :=
+  @[simp] theorem fromBundled.coe {α β : U} (F : α ⟶' β) : funCoe (fromBundled F) = F.f :=
   congrArg BundledFunctor.f (toFromBundled F)
 
-  @[simp] theorem fromBundled.eff {α β : V} (F : α ⟶' β) (a : α) : (fromBundled F) a = F a :=
+  @[simp] theorem fromBundled.eff {α β : U} (F : α ⟶' β) (a : α) : (fromBundled F) a = F a :=
   congrFun (fromBundled.coe F) a
 
   -- We need this to make type class resolution work in some places.
-  @[reducible] def Fun' (α β : V) : V := α ⟶ β
-  notation:20 α:21 " ⟶{" W:0 "} " β:21 => HasFun.Fun' (V := W) α β
+  @[reducible] def Fun' (α β : U) : U := α ⟶ β
+  notation:20 α:21 " ⟶{" V:0 "} " β:20 => HasInternalFunctors.Fun' (U := V) α β
+  instance (α β : U) : CoeFun ⌈α ⟶{U} β⌉ (λ _ => α → β) := ⟨funCoe⟩
 
-  def mkFun' {α β : V} {f : α → β} (hf : h.IsFun f) : α ⟶' β := ⟨f, hf⟩
-  def mkFun  {α β : V} {f : α → β} (hf : h.IsFun f) : α ⟶  β := fromBundled (mkFun' hf)
+  def mkFun' {α β : U} {f : α → β} (hf : h.IsFun f) : α ⟶' β := ⟨f, hf⟩
+  def mkFun  {α β : U} {f : α → β} (hf : h.IsFun f) : α ⟶  β := fromBundled (mkFun' hf)
 
-  @[simp] theorem mkFun.eff {α β : V} {f : α → β} (hf : h.IsFun f) (a : α) :
+  @[simp] theorem mkFun.eff {α β : U} {f : α → β} (hf : h.IsFun f) (a : α) :
     (mkFun hf) a = f a :=
   fromBundled.eff (mkFun' hf) a
 
-end HasFun
+end HasInternalFunctors
 
 -- The following axioms are equivalent to asserting the existence of five functors with specified behavior:
 -- id    : `α ⟶ α,                           a ↦ a`
@@ -205,110 +232,94 @@ end HasFun
 -- subst : `(α ⟶ β ⟶ γ) ⟶ (α ⟶ β) ⟶ (α ⟶ γ), F ↦ (G ↦ (a ↦ F a (G a)))`
 -- from these axioms, and give a general algorithm for proving that a function is functorial.
 
-class HasFunOp (V : Sort v) [h : HasFun V] where
-(idIsFun         (α : V)                               : h.IsFun (λ a : α         => a))
-(constIsFun      (α : V) {β : V} (c : β)               : h.IsFun (λ a : α         => c))
-(constFunIsFun   (α β : V)                             : h.IsFun (λ c : β         => HasFun.mkFun (constIsFun α c)))
-(appIsFun        {α : V} (a : α) (β : V)               : h.IsFun (λ F : α ⟶ β     => F a))
-(appFunIsFun     (α β : V)                             : h.IsFun (λ a : α         => HasFun.mkFun (appIsFun a β)))
-(dupIsFun        {α β : V} (F : α ⟶' α ⟶ β)            : h.IsFun (λ a : α         => F a a))
-(dupFunIsFun     (α β : V)                             : h.IsFun (λ F : α ⟶ α ⟶ β => HasFun.mkFun (dupIsFun (HasFun.toBundled F))))
-(compIsFun       {α β γ : V} (F : α ⟶' β) (G : β ⟶' γ) : h.IsFun (λ a : α         => G (F a)))
-(compFunIsFun    {α β : V} (F : α ⟶' β) (γ : V)        : h.IsFun (λ G : β ⟶ γ     => HasFun.mkFun (compIsFun F (HasFun.toBundled G))))
-(compFunFunIsFun (α β γ : V)                           : h.IsFun (λ F : α ⟶ β     => HasFun.mkFun (compFunIsFun (HasFun.toBundled F) γ)))
+class HasIdFun (U : Universe) [h : HasExternalFunctors U U] where
+(idIsFun (α : U) : h.IsFun (λ a : α => a))
+
+class HasConstFun (U V : Universe) [h : HasExternalFunctors U V] where
+(constIsFun (α : U) {β : V} (c : β) : h.IsFun (λ a : α => c))
+
+class HasCompFun (U V W : Universe) [HasExternalFunctors U V] [HasExternalFunctors V W] [h : HasExternalFunctors U W] where
+(compIsFun {α : U} {β : V} {γ : W} (F : α ⟶' β) (G : β ⟶' γ) : h.IsFun (λ a : α => G (F a)))
+
+class HasExternalFunOp (U : Universe) [h : HasExternalFunctors U U] extends HasIdFun U, HasConstFun U U, HasCompFun U U U
+
+class HasInternalFunOp (U : Universe) [h : HasInternalFunctors U] extends HasExternalFunOp U where
+(constFunIsFun   (α β : U)                      : h.IsFun (λ c : β         => HasInternalFunctors.mkFun (constIsFun α c)))
+(appIsFun        {α : U} (a : α) (β : U)        : h.IsFun (λ F : α ⟶ β     => F a))
+(appFunIsFun     (α β : U)                      : h.IsFun (λ a : α         => HasInternalFunctors.mkFun (appIsFun a β)))
+(dupIsFun        {α β : U} (F : α ⟶' α ⟶ β)     : h.IsFun (λ a : α         => (F a)⟮a⟯))
+(dupFunIsFun     (α β : U)                      : h.IsFun (λ F : α ⟶ α ⟶ β => HasInternalFunctors.mkFun (dupIsFun (HasInternalFunctors.toBundled F))))
+(compFunIsFun    {α β : U} (F : α ⟶' β) (γ : U) : h.IsFun (λ G : β ⟶ γ     => HasInternalFunctors.mkFun (compIsFun F (HasInternalFunctors.toBundled G))))
+(compFunFunIsFun (α β γ : U)                    : h.IsFun (λ F : α ⟶ β     => HasInternalFunctors.mkFun (compFunIsFun (HasInternalFunctors.toBundled F) γ)))
+
+class HasFunOp (U : Universe) extends HasInternalFunctors U, HasInternalFunOp U
 
 namespace HasFunOp
 
-  variable {V : Sort v} [HasFun V] [h : HasFunOp V]
+  variable {U : Universe} [h : HasFunOp U]
 
-  instance : HasFunOp (            V             (⟶)             V            ) := h
-  instance : HasFunOp (            V             (⟶) (    V     (⟶)     V    )) := h
-  instance : HasFunOp ((    V     (⟶)     V    ) (⟶)             V            ) := h
-  instance : HasFunOp ((    V     (⟶)     V    ) (⟶) (    V     (⟶)     V    )) := h
-  instance : HasFunOp (            V             (⟶) (    V     (⟶) (V (⟶) V))) := h
-  instance : HasFunOp ((    V     (⟶)     V    ) (⟶) (    V     (⟶) (V (⟶) V))) := h
-  instance : HasFunOp (            V             (⟶) ((V (⟶) V) (⟶)     V    )) := h
-  instance : HasFunOp (            V             (⟶) ((V (⟶) V) (⟶) (V (⟶) V))) := h
-  instance : HasFunOp ((    V     (⟶)     V    ) (⟶) ((V (⟶) V) (⟶)     V    )) := h
-  instance : HasFunOp ((    V     (⟶)     V    ) (⟶) ((V (⟶) V) (⟶) (V (⟶) V))) := h
-  instance : HasFunOp ((    V     (⟶) (V (⟶) V)) (⟶)             V            ) := h
-  instance : HasFunOp ((    V     (⟶) (V (⟶) V)) (⟶) (    V     (⟶)     V    )) := h
-  instance : HasFunOp ((    V     (⟶) (V (⟶) V)) (⟶) (    V     (⟶) (V (⟶) V))) := h
-  instance : HasFunOp ((    V     (⟶) (V (⟶) V)) (⟶) ((V (⟶) V) (⟶)     V    )) := h
-  instance : HasFunOp ((    V     (⟶) (V (⟶) V)) (⟶) ((V (⟶) V) (⟶) (V (⟶) V))) := h
-  instance : HasFunOp (((V (⟶) V) (⟶)     V    ) (⟶)             V            ) := h
-  instance : HasFunOp (((V (⟶) V) (⟶)     V    ) (⟶) (    V     (⟶)     V    )) := h
-  instance : HasFunOp (((V (⟶) V) (⟶)     V    ) (⟶) (    V     (⟶) (V (⟶) V))) := h
-  instance : HasFunOp (((V (⟶) V) (⟶)     V    ) (⟶) ((V (⟶) V) (⟶)     V    )) := h
-  instance : HasFunOp (((V (⟶) V) (⟶)     V    ) (⟶) ((V (⟶) V) (⟶) (V (⟶) V))) := h
-  instance : HasFunOp (((V (⟶) V) (⟶) (V (⟶) V)) (⟶)             V            ) := h
-  instance : HasFunOp (((V (⟶) V) (⟶) (V (⟶) V)) (⟶) (    V     (⟶)     V    )) := h
-  instance : HasFunOp (((V (⟶) V) (⟶) (V (⟶) V)) (⟶) (    V     (⟶) (V (⟶) V))) := h
-  instance : HasFunOp (((V (⟶) V) (⟶) (V (⟶) V)) (⟶) ((V (⟶) V) (⟶)     V    )) := h
-  instance : HasFunOp (((V (⟶) V) (⟶) (V (⟶) V)) (⟶) ((V (⟶) V) (⟶) (V (⟶) V))) := h
+  def idFun' (α : U) : α ⟶' α := HasInternalFunctors.mkFun' (h.idIsFun α)
+  def idFun  (α : U) : α ⟶  α := HasInternalFunctors.mkFun  (h.idIsFun α)
 
-  def idFun' (α : V) : α ⟶' α := HasFun.mkFun' (h.idIsFun α)
-  def idFun  (α : V) : α ⟶  α := HasFun.mkFun  (h.idIsFun α)
+  @[simp] theorem idFun.eff (α : U) (a : α) : (idFun α) a = a :=
+  by apply HasInternalFunctors.mkFun.eff
 
-  @[simp] theorem idFun.eff (α : V) (a : α) : (idFun α) a = a :=
-  by apply HasFun.mkFun.eff
+  def constFun' (α : U) {β : U} (c : β) : α ⟶' β := HasInternalFunctors.mkFun' (h.constIsFun α c)
+  def constFun  (α : U) {β : U} (c : β) : α ⟶  β := HasInternalFunctors.mkFun  (h.constIsFun α c)
 
-  def constFun' (α : V) {β : V} (c : β) : α ⟶' β := HasFun.mkFun' (h.constIsFun α c)
-  def constFun  (α : V) {β : V} (c : β) : α ⟶  β := HasFun.mkFun  (h.constIsFun α c)
+  @[simp] theorem constFun.eff (α : U) {β : U} (c : β) (a : α) : (constFun α c) a = c :=
+  by apply HasInternalFunctors.mkFun.eff
 
-  @[simp] theorem constFun.eff (α : V) {β : V} (c : β) (a : α) : (constFun α c) a = c :=
-  by apply HasFun.mkFun.eff
+  def constFunFun' (α β : U) : β ⟶' (α ⟶ β) := HasInternalFunctors.mkFun' (h.constFunIsFun α β)
+  def constFunFun  (α β : U) : β ⟶  (α ⟶ β) := HasInternalFunctors.mkFun  (h.constFunIsFun α β)
 
-  def constFunFun' (α β : V) : β ⟶' (α ⟶ β) := HasFun.mkFun' (h.constFunIsFun α β)
-  def constFunFun  (α β : V) : β ⟶  (α ⟶ β) := HasFun.mkFun  (h.constFunIsFun α β)
+  @[simp] theorem constFunFun.eff (α β : U) (c : β) : (constFunFun α β)⟮c⟯ = constFun α c :=
+  by apply HasInternalFunctors.mkFun.eff
 
-  @[simp] theorem constFunFun.eff (α β : V) (c : β) : (constFunFun α β) c = constFun α c :=
-  by apply HasFun.mkFun.eff
+  def appFun' {α : U} (a : α) (β : U) : (α ⟶ β) ⟶' β := HasInternalFunctors.mkFun' (h.appIsFun a β)
+  def appFun  {α : U} (a : α) (β : U) : (α ⟶ β) ⟶  β := HasInternalFunctors.mkFun  (h.appIsFun a β)
 
-  def appFun' {α : V} (a : α) (β : V) : (α ⟶ β) ⟶' β := HasFun.mkFun' (h.appIsFun a β)
-  def appFun  {α : V} (a : α) (β : V) : (α ⟶ β) ⟶  β := HasFun.mkFun  (h.appIsFun a β)
+  @[simp] theorem appFun.eff {α : U} (a : α) (β : U) (F : α ⟶ β) : (appFun a β)⟮F⟯ = F a :=
+  by apply HasInternalFunctors.mkFun.eff
 
-  @[simp] theorem appFun.eff {α : V} (a : α) (β : V) (F : α ⟶ β) : (appFun a β) F = F a :=
-  by apply HasFun.mkFun.eff
+  def appFunFun' (α β : U) : α ⟶' (α ⟶ β) ⟶ β := HasInternalFunctors.mkFun' (h.appFunIsFun α β)
+  def appFunFun  (α β : U) : α ⟶  (α ⟶ β) ⟶ β := HasInternalFunctors.mkFun  (h.appFunIsFun α β)
 
-  def appFunFun' (α β : V) : α ⟶' (α ⟶ β) ⟶ β := HasFun.mkFun' (h.appFunIsFun α β)
-  def appFunFun  (α β : V) : α ⟶  (α ⟶ β) ⟶ β := HasFun.mkFun  (h.appFunIsFun α β)
+  @[simp] theorem appFunFun.eff (α β : U) (a : α) : (appFunFun α β)⟮a⟯ = appFun a β :=
+  by apply HasInternalFunctors.mkFun.eff
 
-  @[simp] theorem appFunFun.eff (α β : V) (a : α) : (appFunFun α β) a = appFun a β :=
-  by apply HasFun.mkFun.eff
+  def dupFun' {α β : U} (F : α ⟶' α ⟶ β) : α ⟶' β := HasInternalFunctors.mkFun' (h.dupIsFun F)
+  def dupFun  {α β : U} (F : α ⟶  α ⟶ β) : α ⟶  β := HasInternalFunctors.mkFun  (h.dupIsFun (HasInternalFunctors.toBundled F))
 
-  def dupFun' {α β : V} (F : α ⟶' α ⟶ β) : α ⟶' β := HasFun.mkFun' (h.dupIsFun F)
-  def dupFun  {α β : V} (F : α ⟶  α ⟶ β) : α ⟶  β := HasFun.mkFun  (h.dupIsFun (HasFun.toBundled F))
+  @[simp] theorem dupFun.eff {α β : U} (F : α ⟶ α ⟶ β) (a : α) : (dupFun F) a = (F⟮a⟯)⟮a⟯ :=
+  by apply HasInternalFunctors.mkFun.eff
 
-  @[simp] theorem dupFun.eff {α β : V} (F : α ⟶ α ⟶ β) (a : α) : (dupFun F) a = F a a :=
-  by apply HasFun.mkFun.eff
+  def dupFunFun' (α β : U) : (α ⟶ α ⟶ β) ⟶' (α ⟶ β) := HasInternalFunctors.mkFun' (h.dupFunIsFun α β)
+  def dupFunFun  (α β : U) : (α ⟶ α ⟶ β) ⟶  (α ⟶ β) := HasInternalFunctors.mkFun  (h.dupFunIsFun α β)
 
-  def dupFunFun' (α β : V) : (α ⟶ α ⟶ β) ⟶' (α ⟶ β) := HasFun.mkFun' (h.dupFunIsFun α β)
-  def dupFunFun  (α β : V) : (α ⟶ α ⟶ β) ⟶  (α ⟶ β) := HasFun.mkFun  (h.dupFunIsFun α β)
+  @[simp] theorem dupFunFun.eff (α β : U) (F : α ⟶ α ⟶ β) : (dupFunFun α β)⟮F⟯ = dupFun F :=
+  by apply HasInternalFunctors.mkFun.eff
 
-  @[simp] theorem dupFunFun.eff (α β : V) (F : α ⟶ α ⟶ β) : (dupFunFun α β) F = dupFun F :=
-  by apply HasFun.mkFun.eff
+  def compFun' {α β γ : U} (F : α ⟶' β) (G : β ⟶' γ) : α ⟶' γ := HasInternalFunctors.mkFun' (h.compIsFun F                                 G)
+  def compFun  {α β γ : U} (F : α ⟶  β) (G : β ⟶  γ) : α ⟶  γ := HasInternalFunctors.mkFun  (h.compIsFun (HasInternalFunctors.toBundled F) (HasInternalFunctors.toBundled G))
 
-  def compFun' {α β γ : V} (F : α ⟶' β) (G : β ⟶' γ) : α ⟶' γ := HasFun.mkFun' (h.compIsFun F                    G)
-  def compFun  {α β γ : V} (F : α ⟶  β) (G : β ⟶  γ) : α ⟶  γ := HasFun.mkFun  (h.compIsFun (HasFun.toBundled F) (HasFun.toBundled G))
+  @[simp] theorem compFun.eff {α β γ : U} (F : α ⟶ β) (G : β ⟶ γ) (a : α) : (compFun F G) a = G (F a) :=
+  by apply HasInternalFunctors.mkFun.eff
 
-  @[simp] theorem compFun.eff {α β γ : V} (F : α ⟶ β) (G : β ⟶ γ) (a : α) : (compFun F G) a = G (F a) :=
-  by apply HasFun.mkFun.eff
+  def compFunFun' {α β : U} (F : α ⟶' β) (γ : U) : (β ⟶ γ) ⟶' (α ⟶ γ) := HasInternalFunctors.mkFun' (h.compFunIsFun F                                 γ)
+  def compFunFun  {α β : U} (F : α ⟶  β) (γ : U) : (β ⟶ γ) ⟶  (α ⟶ γ) := HasInternalFunctors.mkFun  (h.compFunIsFun (HasInternalFunctors.toBundled F) γ)
 
-  def compFunFun' {α β : V} (F : α ⟶' β) (γ : V) : (β ⟶ γ) ⟶' (α ⟶ γ) := HasFun.mkFun' (h.compFunIsFun F                    γ)
-  def compFunFun  {α β : V} (F : α ⟶  β) (γ : V) : (β ⟶ γ) ⟶  (α ⟶ γ) := HasFun.mkFun  (h.compFunIsFun (HasFun.toBundled F) γ)
+  @[simp] theorem compFunFun.eff {α β : U} (F : α ⟶ β) (γ : U) (G : β ⟶ γ) : (compFunFun F γ)⟮G⟯ = compFun F G :=
+  by apply HasInternalFunctors.mkFun.eff
 
-  @[simp] theorem compFunFun.eff {α β : V} (F : α ⟶ β) (γ : V) (G : β ⟶ γ) : (compFunFun F γ) G = compFun F G :=
-  by apply HasFun.mkFun.eff
-
-  def compFunFunFun' (α β γ : V) : (α ⟶ β) ⟶' (β ⟶ γ) ⟶ (α ⟶ γ) := HasFun.mkFun' (h.compFunFunIsFun α β γ)
-  def compFunFunFun  (α β γ : V) : (α ⟶ β) ⟶  (β ⟶ γ) ⟶ (α ⟶ γ) := HasFun.mkFun  (h.compFunFunIsFun α β γ)
+  def compFunFunFun' (α β γ : U) : (α ⟶ β) ⟶' (β ⟶ γ) ⟶ (α ⟶ γ) := HasInternalFunctors.mkFun' (h.compFunFunIsFun α β γ)
+  def compFunFunFun  (α β γ : U) : (α ⟶ β) ⟶  (β ⟶ γ) ⟶ (α ⟶ γ) := HasInternalFunctors.mkFun  (h.compFunFunIsFun α β γ)
   
-  @[simp] theorem compFunFunFun.eff (α β γ : V) (F : α ⟶ β) : (compFunFunFun α β γ) F = compFunFun F γ :=
-  by apply HasFun.mkFun.eff
+  @[simp] theorem compFunFunFun.eff (α β γ : U) (F : α ⟶ β) : (compFunFunFun α β γ)⟮F⟯ = compFunFun F γ :=
+  by apply HasInternalFunctors.mkFun.eff
 
-  def revCompFun' {α β γ : V} (G : β ⟶' γ) (F : α ⟶' β) : α ⟶' γ := compFun' F G
-  def revCompFun  {α β γ : V} (G : β ⟶  γ) (F : α ⟶  β) : α ⟶  γ := compFun  F G
+  def revCompFun' {α β γ : U} (G : β ⟶' γ) (F : α ⟶' β) : α ⟶' γ := compFun' F G
+  def revCompFun  {α β γ : U} (G : β ⟶  γ) (F : α ⟶  β) : α ⟶  γ := compFun  F G
 
   infixr:90 " ⊙' " => revCompFun'
   infixr:90 " ⊙ "  => revCompFun
@@ -323,15 +334,11 @@ end HasFunOp
 
 
 
-class IsKind (V : Sort v) extends HasFun V, HasFunOp V
-
-
-
-def GeneralizedProperty (α : Sort u) (V : Sort v) [HasInstances V] := α → V
+def GeneralizedProperty (α : Sort u) (V : Universe) := α → V
 
 namespace GeneralizedProperty
 
-  variable {α : Sort u} {V : Sort v} [s : HasInstances V]
+  variable {α : Sort u} {V : Universe}
 
   instance hasInstances : HasInstances (GeneralizedProperty α V) := ⟨λ P => ∀ a, P a⟩
 
@@ -362,11 +369,11 @@ open GeneralizedProperty
 -- coerced to a sort. This way, the codomain can be any Lean structure that bundles a sort, in particular
 -- it can be our `Structure` type.
 
-def GeneralizedRelation (α : Sort u) (V : Sort v) [IsKind V] := α → α → V
+def GeneralizedRelation (α : Sort u) (V : Universe) := α → α → V
 
 namespace GeneralizedRelation
 
-  variable {α : Sort u} {V : Sort v} [s : IsKind V]
+  variable {α : Sort u} {V : Universe}
 
   instance hasInstances : HasInstances (GeneralizedRelation α V) := ⟨λ R => ∀ a b, R a b⟩
 
@@ -376,6 +383,8 @@ namespace GeneralizedRelation
 
     class HasRefl  where
     (refl  (a     : α) : R a a)
+
+    variable [HasInternalFunctors V]
 
     class HasSymm  where
     (symm  {a b   : α} : R a b ⟶ R b a)
@@ -388,9 +397,9 @@ namespace GeneralizedRelation
   
   end Properties
 
-  def HasSymm.symm' {R : GeneralizedRelation α V} [h : HasSymm R] {a b : α} (f : R a b) : R b a := h.symm f
-  def HasTrans.trans''  {R : GeneralizedRelation α V} [h : HasTrans R] {a b c : α} (f : R a b) : R b c ⟶ R a c := h.trans f
-  def HasTrans.trans' {R : GeneralizedRelation α V} [h : HasTrans R] {a b c : α} (f : R a b) (g : R b c) : R a c := trans'' f g
+  def HasSymm.symm'    {R : GeneralizedRelation α V} [HasInternalFunctors V] [h : HasSymm  R] {a b   : α} (f : R a b) : R b a := h.symm⟮f⟯
+  def HasTrans.trans'' {R : GeneralizedRelation α V} [HasInternalFunctors V] [h : HasTrans R] {a b c : α} (f : R a b) : R b c ⟶ R a c := h.trans⟮f⟯
+  def HasTrans.trans'  {R : GeneralizedRelation α V} [HasInternalFunctors V] [h : HasTrans R] {a b c : α} (f : R a b) (g : R b c) : R a c := (trans'' f)⟮g⟯
 
   -- When reasoning about instances of `R a b`, we would like to write `trans` as composition, `refl` as
   -- identity, and `symm` as inverse.
@@ -398,12 +407,12 @@ namespace GeneralizedRelation
 
   section Notation
 
-    def revComp {R : GeneralizedRelation α V} [HasTrans R] {a b c : α} (g : R b c) (f : R a b) := HasTrans.trans' f g
+    def revComp {R : GeneralizedRelation α V} [HasInternalFunctors V] [HasTrans R] {a b c : α} (g : R b c) (f : R a b) : R a c := HasTrans.trans' f g
     infixr:90 " • " => revComp
 
     def ident (R : GeneralizedRelation α V) [HasRefl R] (a : α) : R a a := HasRefl.refl a
 
-    def inv {R : GeneralizedRelation α V} [HasSymm R] {a b : α} (f : R a b) := HasSymm.symm' f
+    def inv {R : GeneralizedRelation α V} [HasInternalFunctors V] [HasSymm R] {a b : α} (f : R a b) : R b a := HasSymm.symm' f
     postfix:max "⁻¹" => inv
 
   end Notation
@@ -414,66 +423,14 @@ open GeneralizedRelation
 
 
 
--- We can attach products, arrows, and/or equivalences to a given sort, in the form of generalized
--- relations satisfying appropriate properties.
+-- TODO: Do we want to more dependent properties and relations to a separate file?
 
-section AttachedRelations
-
-  variable (α : Sort u) (V : Sort v) [s : IsKind V]
-
-  class HasProducts where
-  (Product : GeneralizedRelation α V)
-  [hasSymm : HasSymm Product]
-
-  namespace HasProducts
-    variable [h : HasProducts α V]
-    instance productSymm : HasSymm h.Product := h.hasSymm
-    instance hasProduct : HasProduct α α := ⟨h.Product⟩
-    instance : IsKind (HasProduct.γ α α) := s
-    instance : HasSymm (@HasProduct.Product α α (hasProduct α V)) := h.hasSymm
-  end HasProducts
-
-  class HasArrows where
-  (Arrow      : GeneralizedRelation α V)
-  [isPreorder : IsPreorder Arrow]
-
-  namespace HasArrows
-    variable [h : HasArrows α V]
-    instance arrowPreorder : IsPreorder h.Arrow := h.isPreorder
-    instance hasArrow : HasArrow' α α := ⟨h.Arrow⟩
-    instance : IsKind (HasArrow'.γ α α) := s
-    instance : IsPreorder (@HasArrow'.Arrow α α (hasArrow α V)) := h.isPreorder
-  end HasArrows
-
-  class HasEquivalences where
-  (Equiv   : GeneralizedRelation α V)
-  [isEquiv : IsEquivalence Equiv]
-
-  namespace HasEquivalences
-    variable [h : HasEquivalences α V]
-    instance equivEquivalence : IsEquivalence h.Equiv := h.isEquiv
-    instance hasEquivalence : HasEquivalence α α := ⟨h.Equiv⟩
-    instance : IsKind (HasEquivalence.γ α α) := s
-    instance : IsEquivalence (@HasEquivalence.Equiv α α (hasEquivalence α V)) := h.isEquiv
-  end HasEquivalences
-
-end AttachedRelations
-
-namespace HasEquivalences
-  variable {α : Sort u} {V : Sort v} [IsKind V] (h : HasEquivalences α V)
-  def toHasProducts : HasProducts α V := ⟨h.Equiv⟩
-  def toHasArrows   : HasArrows   α V := ⟨h.Equiv⟩
-end HasEquivalences
-
-
-
-def GeneralizedDependentProperty {U : Sort u} [IsKind U] {V : Sort v} [IsKind V] (P : GeneralizedProperty U V)
-                                 (W : Sort w) [IsKind W] :=
+def GeneralizedDependentProperty {U V : Universe} (P : GeneralizedProperty ⌈U⌉ V) (W : Universe) :=
 ∀ {α}, P α → (α → W)
 
 namespace GeneralizedDependentProperty
 
-  variable {U : Sort u} [IsKind U] {V : Sort v} [IsKind V] {P : GeneralizedProperty U V} {W : Sort w} [IsKind W]
+  variable {U V : Universe} {P : GeneralizedProperty ⌈U⌉ V} {W : Universe}
 
   section Properties
 
@@ -482,7 +439,7 @@ namespace GeneralizedDependentProperty
     class HasDependentInst [h : HasInst P] where
     (inst {α : U} (a : α) : D (h.inst α) a)
 
-    def instProp [h : HasInst P] (α : U) : GeneralizedProperty (HasInstances.Inst α) W := D (h.inst α)
+    def instProp [h : HasInst P] (α : U) : GeneralizedProperty ⌈α⌉ W := D (h.inst α)
     instance [HasInst P] [h : HasDependentInst D] (α : U) : HasInst (instProp D α) := ⟨h.inst⟩
 
   end Properties
@@ -493,13 +450,12 @@ open GeneralizedDependentProperty
 
 
 
-def GeneralizedDependentRelation {U : Sort u} [IsKind U] {V : Sort v} [IsKind V] (R : GeneralizedRelation U V)
-                                 (W : Sort w) [IsKind W] :=
+def GeneralizedDependentRelation {U V : Universe} (R : GeneralizedRelation ⌈U⌉ V) (W : Universe) :=
 ∀ {α β}, R α β → (α → β → W)
 
 namespace GeneralizedDependentRelation
 
-  variable {U : Sort u} [IsKind U] {V : Sort v} [IsKind V] {R : GeneralizedRelation U V} {W : Sort w} [IsKind W]
+  variable {U V : Universe} {R : GeneralizedRelation ⌈U⌉ V} {W : Universe}
 
   section Properties
 
@@ -508,38 +464,45 @@ namespace GeneralizedDependentRelation
     class HasDependentRefl  [h : HasRefl  R] where
     (refl  {α     : U}                         (a : α)                 : D (h.refl α) a a)
 
-    def reflRel [h : HasRefl R] (α : U) : GeneralizedRelation (HasInstances.Inst α) W := D (h.refl α)
+    def reflRel [h : HasRefl R] (α : U) : GeneralizedRelation ⌈α⌉ W := D (h.refl α)
     instance [HasRefl R] [h : HasDependentRefl D] (α : U) : HasRefl (reflRel D α) := ⟨h.refl⟩
 
+    variable [HasInternalFunctors V] [HasInternalFunctors W]
+
     class HasDependentSymm  [h : HasSymm  R] where
-    (symm  {α β   : U} {F : R α β}             {a : α} {b : β}         : D F a b ⟶ D (h.symm F) b a)
+    (symm  {α β   : U} {F : R α β}             {a : α} {b : β}         : D F a b ⟶ D h.symm⟮F⟯ b a)
 
     class HasDependentTrans [h : HasTrans R] where
-    (trans {α β γ : U} {F : R α β} {G : R β γ} {a : α} {b : β} {c : γ} : D F a b ⟶ D G b c ⟶ D (h.trans F G) a c)
+    (trans {α β γ : U} {F : R α β} {G : R β γ} {a : α} {b : β} {c : γ} : D F a b ⟶ D G b c ⟶ D h.trans⟮F⟯⟮G⟯ a c)
 
     class IsDependentPreorder    [h : IsPreorder    R] extends HasDependentRefl D, HasDependentTrans D
     class IsDependentEquivalence [h : IsEquivalence R] extends IsDependentPreorder D, HasDependentSymm D
 
   end Properties
 
-  def HasDependentSymm.symm' {D : GeneralizedDependentRelation R W} [HasSymm R] [h : HasDependentSymm D] {α β : U}
-                             {F : R α β} {a : α} {b : β} (f : D F a b) : D (HasSymm.symm' F) b a :=
-  h.symm f
+  def HasDependentSymm.symm'    {D : GeneralizedDependentRelation R W}
+                                [HasInternalFunctors V] [HasInternalFunctors W] [HasSymm  R] [h : HasDependentSymm  D]
+                                {α β : U} {F : R α β} {a : α} {b : β} (f : D F a b) :
+   D (HasSymm.symm' F) b a :=
+  h.symm⟮f⟯
 
-  def HasDependentTrans.trans'' {D : GeneralizedDependentRelation R W} [HasTrans R] [h : HasDependentTrans D] {α β γ : U}
-                                {F : R α β} {G : R β γ} {a : α} {b : β} {c : γ} (f : D F a b) :
+  def HasDependentTrans.trans'' {D : GeneralizedDependentRelation R W}
+                                [HasInternalFunctors V] [HasInternalFunctors W] [HasTrans R] [h : HasDependentTrans D]
+                                {α β γ : U} {F : R α β} {G : R β γ} {a : α} {b : β} {c : γ} (f : D F a b) :
     D G b c ⟶ D (HasTrans.trans' F G) a c :=
-  h.trans f
+  h.trans⟮f⟯
 
-  def HasDependentTrans.trans'  {D : GeneralizedDependentRelation R W} [HasTrans R] [h : HasDependentTrans D] {α β γ : U}
-                                {F : R α β} {G : R β γ} {a : α} {b : β} {c : γ} (f : D F a b) (g : D G b c) :
-    D (HasTrans.trans' F G) a c
-  := h.trans f g
+  def HasDependentTrans.trans'  {D : GeneralizedDependentRelation R W}
+                                [HasInternalFunctors V] [HasInternalFunctors W] [HasTrans R] [h : HasDependentTrans D]
+                                {α β γ : U} {F : R α β} {G : R β γ} {a : α} {b : β} {c : γ} (f : D F a b) (g : D G b c) :
+    D (HasTrans.trans' F G) a c :=
+  (trans'' f)⟮g⟯
 
   section Notation
 
-    def depRevComp {D : GeneralizedDependentRelation R W} [HasTrans R] [HasDependentTrans D] {α β γ : U}
-                   {F : R α β} {G : R β γ} {a : α} {b : β} {c : γ} (g : D G b c) (f : D F a b) :
+    def depRevComp {D : GeneralizedDependentRelation R W} [HasInternalFunctors V] [HasInternalFunctors W]
+                   [HasTrans R] [HasDependentTrans D]
+                   {α β γ : U} {F : R α β} {G : R β γ} {a : α} {b : β} {c : γ} (g : D G b c) (f : D F a b) :
       D (G • F) a c :=
     HasDependentTrans.trans' f g
     -- TODO: What is the correct way to overload this?
@@ -549,8 +512,9 @@ namespace GeneralizedDependentRelation
       D (ident R α) a a :=
     HasDependentRefl.refl a
 
-    def depInv {D : GeneralizedDependentRelation R W} [HasSymm R] [HasDependentSymm D] {α β : U}
-               {F : R α β} {a : α} {b : β} (f : D F a b) :
+    def depInv {D : GeneralizedDependentRelation R W} [HasInternalFunctors V] [HasInternalFunctors W]
+               [HasSymm R] [HasDependentSymm D]
+               {α β : U} {F : R α β} {a : α} {b : β} (f : D F a b) :
       D F⁻¹ b a :=
     HasDependentSymm.symm' f
     --postfix:max "⁻¹" => depInv
@@ -563,41 +527,106 @@ open GeneralizedDependentRelation
 
 
 
+section Sets
+
+  variable (M : Universe)
+
+  -- TODO: We want sets to have an instance equivalence (i.e. equality).
+  -- For this, we probably need to start with a universe with instance equivalences.
+  -- I think we need to introduce a `UniverseWithEquivalences` type. Or is it just `Groupoid`?
+
+  def Subset (U : Universe) := GeneralizedProperty ⌈U⌉ M
+
+  @[reducible] def GeneralizedSet := Bundled (Subset M)
+
+  def setUniverse : Universe := ⟨GeneralizedSet M⟩
+
+end Sets
+
+
+
+-- We can attach products, arrows, and/or equivalences to a given sort, in the form of generalized
+-- relations satisfying appropriate properties.
+
+section AttachedRelations
+
+  variable (α : Sort u) (V : Universe) [HasInternalFunctors V]
+
+  class HasProducts where
+  (Product : GeneralizedRelation α V)
+  [hasSymm : HasSymm Product]
+
+  namespace HasProducts
+    variable [h : HasProducts α V]
+    instance productSymm : HasSymm h.Product := h.hasSymm
+    instance hasProduct : HasProduct α α := ⟨h.Product⟩
+    instance : HasInstances (HasProduct.γ α α) := Universe.instInst V
+    instance : HasSymm (@HasProduct.Product α α (hasProduct α V)) := h.hasSymm
+  end HasProducts
+
+  class HasArrows where
+  (Arrow      : GeneralizedRelation α V)
+  [isPreorder : IsPreorder Arrow]
+
+  namespace HasArrows
+    variable [h : HasArrows α V]
+    instance arrowPreorder : IsPreorder h.Arrow := h.isPreorder
+    instance hasArrow : HasArrow' α α := ⟨h.Arrow⟩
+    instance : HasInstances (HasArrow'.γ α α) := Universe.instInst V
+    instance : IsPreorder (@HasArrow'.Arrow α α (hasArrow α V)) := h.isPreorder
+  end HasArrows
+
+  class HasEquivalences where
+  (Equiv   : GeneralizedRelation α V)
+  [isEquiv : IsEquivalence Equiv]
+
+  namespace HasEquivalences
+    variable [h : HasEquivalences α V]
+    instance equivEquivalence : IsEquivalence h.Equiv := h.isEquiv
+    instance hasEquivalence : HasEquivalence α α := ⟨h.Equiv⟩
+    instance : HasInstances (HasEquivalence.γ α α) := Universe.instInst V
+    instance : IsEquivalence (@HasEquivalence.Equiv α α (hasEquivalence α V)) := h.isEquiv
+  end HasEquivalences
+
+end AttachedRelations
+
+
+
 section AttachedDependentRelations
 
-  variable (U : Sort u) [IsKind U] (V : Sort v) [IsKind V] (W : Sort w) [IsKind W]
+  variable (U V W : Universe) [HasInternalFunctors V] [HasInternalFunctors W]
 
-  class HasDependentProducts [h : HasProducts U V] where
+  class HasDependentProducts [h : HasProducts ⌈U⌉ V] where
   (Product : GeneralizedDependentRelation h.Product W)
   [hasSymm : HasDependentSymm Product]
 
   namespace HasDependentProducts
-    variable [HasProducts U V] [h : HasDependentProducts U V W]
+    variable [HasProducts ⌈U⌉ V] [h : HasDependentProducts U V W]
     instance productSymm : HasDependentSymm h.Product := h.hasSymm
     notation:35 a:36 " ⊓[" P:0 "] " b:36 => HasDependentProducts.Product P a b
-    notation:35 a:36 " ⊓[" P:0 "," V:0 "," W:0 "] " b:36 => HasDependentProducts.Product (V := V) (W := W) P a b
+    notation:35 a:36 " ⊓[" P:0 "," V':0 "," W':0 "] " b:36 => HasDependentProducts.Product (V := V') (W := W') P a b
   end HasDependentProducts
 
-  class HasDependentArrows [h : HasArrows U V] where
+  class HasDependentArrows [h : HasArrows ⌈U⌉ V] where
   (Arrow      : GeneralizedDependentRelation h.Arrow W)
   [isPreorder : IsDependentPreorder Arrow]
 
   namespace HasDependentArrows
-    variable [HasArrows U V] [h : HasDependentArrows U V W]
+    variable [HasArrows ⌈U⌉ V] [h : HasDependentArrows U V W]
     instance arrowPreorder : IsDependentPreorder h.Arrow := h.isPreorder
     notation:20 a:21 " ⇝[" F:0 "] " b:21 => HasDependentArrows.Arrow F a b
-    notation:20 a:21 " ⇝[" F:0 "," V:0 "," W:0 "] " b:21 => HasDependentArrows.Arrow (V := V) (W := W) F a b
+    notation:20 a:21 " ⇝[" F:0 "," V':0 "," W':0 "] " b:21 => HasDependentArrows.Arrow (V := V') (W := W') F a b
   end HasDependentArrows
 
-  class HasDependentEquivalences [h : HasEquivalences U V] where
+  class HasDependentEquivalences [h : HasEquivalences ⌈U⌉ V] where
   (Equiv   : GeneralizedDependentRelation h.Equiv W)
   [isEquiv : IsDependentEquivalence Equiv]
 
   namespace HasDependentEquivalences
-    variable [HasEquivalences U V] [h : HasDependentEquivalences U V W]
+    variable [HasEquivalences ⌈U⌉ V] [h : HasDependentEquivalences U V W]
     instance equivEquivalence : IsDependentEquivalence h.Equiv := h.isEquiv
     notation:25 a:26 " ≃[" F:0 "] " b:26 => HasDependentEquivalences.Equiv F a b
-    notation:25 a:26 " ≃[" F:0 "," V:0 "," W:0 "] " b:26 => HasDependentEquivalences.Equiv (V := V) (W := W) F a b
+    notation:25 a:26 " ≃[" F:0 "," V':0 "," W':0 "] " b:26 => HasDependentEquivalences.Equiv (V := V') (W := W') F a b
   end HasDependentEquivalences
 
 end AttachedDependentRelations
@@ -611,85 +640,78 @@ end AttachedDependentRelations
 --
 -- TODO: describe arrows
 
-class HasInstanceArrows (V : Sort v) [s : IsKind V] where
-(ArrowKind                                    : Sort w)
-[arrowIsKind                                  : IsKind ArrowKind]
-[hasArrows (α : V)                            : HasArrows (s.Inst α) ArrowKind]
-(arrowCongr {α β : V} {F G : α ⟶ β} {a b : α} : (hasArrows (α ⟶ β)).Arrow F G ⟶
-                                                (hasArrows α).Arrow a b ⟶
-                                                (hasArrows β).Arrow (F a) (G b))
+class HasInstanceArrows (U : Universe) where
+(arrowUniverse           : Universe)
+[arrowHasFunOp           : HasFunOp arrowUniverse]
+(Arrow (α : U)           : GeneralizedRelation ⌈α⌉ arrowUniverse)
+[arrowIsPreorder (α : U) : IsPreorder (Arrow α)]
 
 namespace HasInstanceArrows
 
-  variable (V : Sort v) [s : IsKind V] [h : HasInstanceArrows V]
+  variable (U : Universe) [h : HasInstanceArrows U]
 
-  instance arrowKind : IsKind h.ArrowKind := h.arrowIsKind
-  instance instArrows (α : V) : HasArrows (s.Inst α) h.ArrowKind := h.hasArrows α
-  def InstArrow (α : V) : GeneralizedRelation (s.Inst α) h.ArrowKind := (instArrows V α).Arrow
+  instance hasFunOp : HasFunOp h.arrowUniverse := h.arrowHasFunOp
 
-  @[reducible] def InstArrowType (α : V) := s.Inst α (⇝) s.Inst α
+  instance arrowPreorder (α : U) : IsPreorder (h.Arrow α) := h.arrowIsPreorder α
+
+  instance hasArrows (α : U) : HasArrows ⌈α⌉ h.arrowUniverse := ⟨h.Arrow α⟩
+  @[reducible] def InstArrowType (α : U) := ⌈α⌉ (⇝) ⌈α⌉
+  instance (α : U) : HasInstances (InstArrowType U α) := Universe.instInst h.arrowUniverse
 
   -- Again, this is potentially endless...
-  instance (α β     : V) : HasArrow (InstArrowType V α)                (InstArrowType V β)                                    := HasFun.hasArrow
-  instance (α β     : V) : IsKind   (InstArrowType V α (⟶)              InstArrowType V β)                                    := h.arrowIsKind
-  instance (α β γ   : V) : HasArrow (InstArrowType V α)    (InstArrowType V β (⟶)              InstArrowType V γ)             := HasFun.hasArrow
-  instance (α β γ   : V) : IsKind   (InstArrowType V α (⟶) (InstArrowType V β (⟶)              InstArrowType V γ))            := h.arrowIsKind
-  instance (α β γ δ : V) : HasArrow (InstArrowType V α)    (InstArrowType V β (⟶) (InstArrowType V γ (⟶) InstArrowType V δ))  := HasFun.hasArrow
-  instance (α β γ δ : V) : IsKind   (InstArrowType V α (⟶) (InstArrowType V β (⟶) (InstArrowType V γ (⟶) InstArrowType V δ))) := h.arrowIsKind
-
-  def arrCongr {α β : V} {F G : α ⟶{V} β} {a b : α} : (F ⇝ G) ⟶ (a ⇝ b) ⟶ (F a ⇝ G b) := h.arrowCongr
+  instance (α β     : U) : HasArrow (InstArrowType U α)             (InstArrowType U β)                                   := HasInternalFunctors.hasArrow
+  instance (α β γ   : U) : HasArrow (InstArrowType U α) (InstArrowType U β (⟶)              InstArrowType U γ)            := HasInternalFunctors.hasArrow
+  instance (α β γ δ : U) : HasArrow (InstArrowType U α) (InstArrowType U β (⟶) (InstArrowType U γ (⟶) InstArrowType U δ)) := HasInternalFunctors.hasArrow
 
 end HasInstanceArrows
 
-class HasInstanceEquivalences (V : Sort v) [s : IsKind V] extends HasInstanceArrows V where
-[arrowSymm (α : V) : HasSymm (hasArrows α).Arrow]
+class HasFunctorialArrows (U : Universe) [HasInternalFunctors U] extends HasInstanceArrows U where
+(arrowCongr {α β : U} {F G : α ⟶{U} β} {a b : α} : (F ⇝ G) ⟶{arrowUniverse} (a ⇝ b) ⟶ (F a ⇝ G b))
+
+class HasInstanceEquivalences (U : Universe) where
+(equivUniverse              : Universe)
+[equivHasFunOp              : HasFunOp equivUniverse]
+(Equiv (α : U)              : GeneralizedRelation ⌈α⌉ equivUniverse)
+[equivIsEquivalence (α : U) : IsEquivalence (Equiv α)]
 
 namespace HasInstanceEquivalences
 
-  variable (V : Sort v) [s : IsKind V] [h : HasInstanceEquivalences V]
+  variable (U : Universe) [h : HasInstanceEquivalences U]
 
-  instance (α : V) : HasSymm (h.hasArrows α).Arrow := h.arrowSymm α
-  instance arrowIsEquiv (α : V) : IsEquivalence (h.hasArrows α).Arrow := ⟨⟩
-  instance instEquivs (α : V) : HasEquivalences (s.Inst α) h.ArrowKind := ⟨(h.hasArrows α).Arrow⟩
+  instance hasFunOp : HasFunOp h.equivUniverse := h.equivHasFunOp
 
-  @[reducible] def InstEquivType (α : V) := s.Inst α (≃) s.Inst α
+  instance equivEquivalence (α : U) : IsEquivalence (h.Equiv α) := h.equivIsEquivalence α
+
+  instance hasEquivalences (α : U) : HasEquivalences ⌈α⌉ h.equivUniverse := ⟨h.Equiv α⟩
+  @[reducible] def InstEquivType (α : U) := ⌈α⌉ (≃) ⌈α⌉
+  instance (α : U) : HasInstances (InstEquivType U α) := Universe.instInst h.equivUniverse
 
   -- Again, this is potentially endless...
-  instance (α β     : V) : HasArrow (InstEquivType V α)                (InstEquivType V β)                                    := HasFun.hasArrow
-  instance (α β     : V) : IsKind   (InstEquivType V α (⟶)              InstEquivType V β)                                    := h.arrowIsKind
-  instance (α β γ   : V) : HasArrow (InstEquivType V α)    (InstEquivType V β (⟶)              InstEquivType V γ)             := HasFun.hasArrow
-  instance (α β γ   : V) : IsKind   (InstEquivType V α (⟶) (InstEquivType V β (⟶)              InstEquivType V γ))            := h.arrowIsKind
-  instance (α β γ δ : V) : HasArrow (InstEquivType V α)    (InstEquivType V β (⟶) (InstEquivType V γ (⟶) InstEquivType V δ))  := HasFun.hasArrow
-  instance (α β γ δ : V) : IsKind   (InstEquivType V α (⟶) (InstEquivType V β (⟶) (InstEquivType V γ (⟶) InstEquivType V δ))) := h.arrowIsKind
+  instance (α β     : U) : HasArrow (InstEquivType U α)             (InstEquivType U β)                                   := HasInternalFunctors.hasArrow
+  instance (α β γ   : U) : HasArrow (InstEquivType U α) (InstEquivType U β (⟶)              InstEquivType U γ)            := HasInternalFunctors.hasArrow
+  instance (α β γ δ : U) : HasArrow (InstEquivType U α) (InstEquivType U β (⟶) (InstEquivType U γ (⟶) InstEquivType U δ)) := HasInternalFunctors.hasArrow
 
-  instance : HasFun V := s.toHasFun
-
-  def funCongr {α β : V} {F G : α ⟶{V} β} {a b : α} : F ≃ G ⟶ a ≃ b ⟶ F a ≃ G b := h.arrowCongr
+  def toHasInstanceArrows : HasInstanceArrows U :=
+  { arrowUniverse   := h.equivUniverse,
+    arrowHasFunOp   := h.equivHasFunOp,
+    Arrow           := h.Equiv,
+    arrowIsPreorder := λ α => (h.equivIsEquivalence α).toIsPreorder }
 
 end HasInstanceEquivalences
 
-class HasInstanceEquivalences' (V : Sort v) [s : IsKind V] where
-(EquivKind                                    : Sort w)
-[equivIsKind                                  : IsKind EquivKind]
-[hasEquivalences (α : V)                      : HasEquivalences (s.Inst α) EquivKind]
-(equivCongr {α β : V} {F G : α ⟶ β} {a b : α} : (hasEquivalences (α ⟶ β)).Equiv F G ⟶
-                                                (hasEquivalences α).Equiv a b ⟶
-                                                (hasEquivalences β).Equiv (F a) (G b))
+class HasFunctorialEquivalences (U : Universe) [HasInternalFunctors U] extends HasInstanceEquivalences U where
+(equivCongr {α β : U} {F G : α ⟶{U} β} {a b : α} : F ≃ G ⟶{equivUniverse} a ≃ b ⟶ F a ≃ G b)
 
-namespace HasInstanceEquivalences'
+namespace HasFunctorialEquivalences
 
-  variable {V : Sort v} [s : IsKind V] [h : HasInstanceEquivalences' V]
+  variable (U : Universe) [HasInternalFunctors U] [h : HasFunctorialEquivalences U]
 
-  instance equivKind : IsKind h.EquivKind := h.equivIsKind
+  def toHasFunctorialArrows : HasFunctorialArrows U :=
+  { toHasInstanceArrows := HasInstanceEquivalences.toHasInstanceArrows U,
+    arrowCongr          := h.equivCongr }
 
-  instance toHasInstancesEquivalences : HasInstanceEquivalences V :=
-  { ArrowKind   := h.EquivKind,
-    arrowIsKind := h.equivIsKind,
-    hasArrows   := λ α => HasEquivalences.toHasArrows (h.hasEquivalences α),
-    arrowCongr  := h.equivCongr,
-    arrowSymm   := λ α => (h.hasEquivalences α).isEquiv.toHasSymm }
+end HasFunctorialEquivalences
 
-end HasInstanceEquivalences'
 
 
 -- We would also like to be able to manipulate such equivalences, and we need them to behave like
@@ -720,26 +742,23 @@ end HasInstanceEquivalences'
 
 section Morphisms
 
-  variable {α : Sort u} {V : Sort v} [IsKind V] [HasInstanceArrows V] (R : GeneralizedRelation α V)
+  variable {α : Sort u} {V : Universe} [HasInternalFunctors V] [hasArrows : HasInstanceArrows V]
+           (R : GeneralizedRelation α V)
 
-  class IsCompositionRelation extends HasTrans R where
+  class IsCompositionRelation [HasTrans      R] where
   (assocLR {a b c d : α} (f : R a b) (g : R b c) (h : R c d) : (h • g) • f ⇝ h • (g • f))
   (assocRL {a b c d : α} (f : R a b) (g : R b c) (h : R c d) : h • (g • f) ⇝ (h • g) • f)
 
-  class IsMorphismRelation extends IsCompositionRelation R, HasRefl R where
+  class IsMorphismRelation    [IsPreorder    R] extends IsCompositionRelation R where
   (leftId  {a b : α} (f : R a b) : ident R b • f ⇝ f)
   (rightId {a b : α} (f : R a b) : f • ident R a ⇝ f)
 
-  instance morPreorder [IsMorphismRelation R] : IsPreorder R := ⟨⟩
-
-  class IsIsomorphismRelation extends IsMorphismRelation R, HasSymm R where
+  class IsIsomorphismRelation [IsEquivalence R] extends IsMorphismRelation R where
   (leftInv  {a b   : α} (f : R a b)             : f⁻¹ • f       ⇝ ident R a)
   (rightInv {a b   : α} (f : R a b)             : f • f⁻¹       ⇝ ident R b)
   (invInv   {a b   : α} (f : R a b)             : (f⁻¹)⁻¹       ⇝ f)
   (compInv  {a b c : α} (f : R a b) (g : R b c) : (g • f)⁻¹     ⇝ f⁻¹ • g⁻¹)
   (idInv    (a     : α)                         : (ident R a)⁻¹ ⇝ ident R a)
-
-  instance isoEquiv [IsIsomorphismRelation R] : IsEquivalence R := ⟨⟩
 
 end Morphisms
 
@@ -747,21 +766,23 @@ end Morphisms
 
 section Functors
 
-  variable {α : Sort u} {V : Sort v} {W : Sort w} [IsKind V] [IsKind W] [HasInstanceArrows W] [HasIsFun V W]
+  variable {α : Sort u} {V W : Universe} [hasArrows : HasInstanceArrows W] [HasExternalFunctors V W]
            (R : GeneralizedRelation α V) (S : GeneralizedRelation α W)
 
   def BaseFunctor := ∀ {a b}, R a b ⟶' S a b
 
   variable (F : BaseFunctor R S)
 
-  class IsReflFunctor  [HasRefl  R] [HasRefl  S] where
-  (respectsRefl  (a     : α)                         : F (ident R a) ⇝ ident S a)
+  class IsReflFunctor  [hR : HasRefl  R] [hS : HasRefl  S] where
+  (respectsRefl  (a     : α)                         : F (hR.refl   a)   ⇝ hS.refl   a)
 
-  class IsSymmFunctor  [HasSymm  R] [HasSymm  S] where
-  (respectsSymm  {a b   : α} (f : R a b)             : F f⁻¹         ⇝ (F f)⁻¹)
+  variable [HasInternalFunctors V] [HasInternalFunctors W]
 
-  class IsTransFunctor [HasTrans R] [HasTrans S] where
-  (respectsTrans {a b c : α} (f : R a b) (g : R b c) : F (g • f)     ⇝ F g • F f)
+  class IsSymmFunctor  [hR : HasSymm  R] [hS : HasSymm  S] where
+  (respectsSymm  {a b   : α} (f : R a b)             : F (hR.symm'  f)   ⇝ hS.symm'  (F f))
+
+  class IsTransFunctor [hR : HasTrans R] [hS : HasTrans S] where
+  (respectsTrans {a b c : α} (f : R a b) (g : R b c) : F (hR.trans' f g) ⇝ hS.trans' (F f) (F g))
 
   class IsPreorderFunctor    [IsPreorder    R] [IsPreorder    S] extends IsReflFunctor R S F, IsTransFunctor R S F
   class IsEquivalenceFunctor [IsEquivalence R] [IsEquivalence S] extends IsPreorderFunctor R S F, IsSymmFunctor R S F
@@ -772,21 +793,16 @@ end Functors
 
 section NaturalTransformations
 
-  variable {α : Sort u} {β : Sort w} {V : Sort v} {W : Sort w} [IsKind V] [IsKind W] [HasInstanceEquivalences W] [HasIsFun V W]
+  variable {α : Sort u} {β : Sort v} {V W : Universe} [HasInternalFunctors W] [hasEquivs : HasInstanceEquivalences W]
+           [HasExternalFunctors V W]
            (R : GeneralizedRelation α V) (S : GeneralizedRelation β W) [h : HasTrans S]
            {mF mG : α → β} (F : ∀ {a b}, R a b ⟶' S (mF a) (mF b)) (G : ∀ {a b}, R a b ⟶' S (mG a) (mG b))
 
-  class IsNaturalTransformation (n : ∀ a, S (mF a) (mG a)) where
-  (nat {a b : α} (f : R a b) : G f • n a ≃ n b • F f)
+  class IsNatural (n : ∀ a, S (mF a) (mG a)) where
+  (nat {a b : α} (f : R a b) : h.trans' (n a) (G f) ≃ h.trans' (F f) (n b))
 
 end NaturalTransformations
 
 
 
 -- TODO: If arrows have equivalences, we can specify redundancies.
-
-
-
-class IsCategory (α : Sort u) {MorphismKind : Sort v} [IsKind MorphismKind] [HasInstanceEquivalences MorphismKind] where
-(M     : GeneralizedRelation α MorphismKind)
-[isMor : IsMorphismRelation M]
