Structure/Generic/Lemmas.lean
@@ -10,6 +10,8 @@
 import Structure.Generic.Axioms
 import mathlib4_experiments.Data.Equiv.Basic
 
+open GeneralizedRelation
+
 
 
 set_option autoBoundImplicitLocal false
@@ -28,141 +30,141 @@ by subst ha; rfl
 
 namespace HasFunOp
 
-  variable {V : Sort v} [HasFun V] [h : HasFunOp V]
+  variable {U : Universe} [h : HasFunOp U]
 
   -- The "swap" functor swaps the arguments of a nested functor. Its plain version `swapFun` actually
   -- just fixes the second argument.
 
-  def swapIsFun {α β γ : V} (F : α ⟶' β ⟶ γ) (b : β) : HasIsFun.IsFun (λ a : α => F a b) :=
+  def swapIsFun {α β γ : U} (F : α ⟶' β ⟶ γ) (b : β) : HasExternalFunctors.IsFun (λ a : α => F a b) :=
   h.compIsFun F (appFun' b γ)
 
-  def swapFun' {α β γ : V} (F : α ⟶' β ⟶ γ) (b : β) : α ⟶' γ := HasFun.mkFun' (swapIsFun F                    b)
-  def swapFun  {α β γ : V} (F : α ⟶  β ⟶ γ) (b : β) : α ⟶  γ := HasFun.mkFun  (swapIsFun (HasFun.toBundled F) b)
+  def swapFun' {α β γ : U} (F : α ⟶' β ⟶ γ) (b : β) : α ⟶' γ := HasInternalFunctors.mkFun' (swapIsFun F                                 b)
+  def swapFun  {α β γ : U} (F : α ⟶  β ⟶ γ) (b : β) : α ⟶  γ := HasInternalFunctors.mkFun  (swapIsFun (HasInternalFunctors.toBundled F) b)
 
-  @[simp] theorem swapFun.eff {α β γ : V} (F : α ⟶ β ⟶ γ) (b : β) (a : α) :
-    (swapFun F b) a = F a b :=
-  by apply HasFun.mkFun.eff
+  @[simp] theorem swapFun.eff {α β γ : U} (F : α ⟶ β ⟶ γ) (b : β) (a : α) :
+    (swapFun F b) a = F⟮a⟯ b :=
+  by apply HasInternalFunctors.mkFun.eff
 
-  theorem swapFunFun.def {α β γ : V} (F : α ⟶' β ⟶ γ) (b : β) :
-    HasFun.mkFun (swapIsFun F b) = HasFun.mkFun (h.compIsFun F (HasFun.toBundled (appFun b γ))) :=
-  HasFun.toFromBundled (appFun' b γ) ▸ rfl
+  theorem swapFunFun.def {α β γ : U} (F : α ⟶' β ⟶ γ) (b : β) :
+    HasInternalFunctors.mkFun (swapIsFun F b) = HasInternalFunctors.mkFun (h.compIsFun F (HasInternalFunctors.toBundled (appFun b γ))) :=
+  HasInternalFunctors.toFromBundled (appFun' b γ) ▸ rfl
 
-  def swapFunIsFun {α β γ : V} (F : α ⟶' β ⟶ γ) : HasIsFun.IsFun (λ b : β => HasFun.mkFun (swapIsFun F b)) :=
+  def swapFunIsFun {α β γ : U} (F : α ⟶' β ⟶ γ) : HasExternalFunctors.IsFun (λ b : β => HasInternalFunctors.mkFun (swapIsFun F b)) :=
   funext (swapFunFun.def F) ▸ h.compIsFun (appFunFun' β γ) (compFunFun' F γ)
 
-  def swapFunFun' {α β γ : V} (F : α ⟶' β ⟶ γ) : β ⟶' α ⟶ γ := HasFun.mkFun' (swapFunIsFun F)
-  def swapFunFun  {α β γ : V} (F : α ⟶  β ⟶ γ) : β ⟶  α ⟶ γ := HasFun.mkFun  (swapFunIsFun (HasFun.toBundled F))
+  def swapFunFun' {α β γ : U} (F : α ⟶' β ⟶ γ) : β ⟶' α ⟶ γ := HasInternalFunctors.mkFun' (swapFunIsFun F)
+  def swapFunFun  {α β γ : U} (F : α ⟶  β ⟶ γ) : β ⟶  α ⟶ γ := HasInternalFunctors.mkFun  (swapFunIsFun (HasInternalFunctors.toBundled F))
 
-  @[simp] theorem swapFunFun.eff {α β γ : V} (F : α ⟶ β ⟶ γ) (b : β) :
-    (swapFunFun F) b = swapFun F b :=
-  by apply HasFun.mkFun.eff
+  @[simp] theorem swapFunFun.eff {α β γ : U} (F : α ⟶ β ⟶ γ) (b : β) :
+    (swapFunFun F)⟮b⟯ = swapFun F b :=
+  by apply HasInternalFunctors.mkFun.eff
 
-  theorem swapFunFunFun.def (α β γ : V) (F : α ⟶ β ⟶ γ) :
-    swapFunFun F = HasFun.mkFun (h.compIsFun (appFunFun' β γ) (HasFun.toBundled (compFunFun F γ))) :=
-  HasFun.toFromBundled (compFunFun' (HasFun.toBundled F) γ) ▸ elimRec
+  theorem swapFunFunFun.def (α β γ : U) (F : α ⟶ β ⟶ γ) :
+    swapFunFun F = HasInternalFunctors.mkFun (h.compIsFun (appFunFun' β γ) (HasInternalFunctors.toBundled (compFunFun F γ))) :=
+  HasInternalFunctors.toFromBundled (compFunFun' (HasInternalFunctors.toBundled F) γ) ▸ elimRec
 
-  def swapFunFunIsFun (α β γ : V) : HasIsFun.IsFun (λ F : α ⟶ β ⟶ γ => swapFunFun F) :=
+  def swapFunFunIsFun (α β γ : U) : HasExternalFunctors.IsFun (λ F : α ⟶ β ⟶ γ => swapFunFun F) :=
   funext (swapFunFunFun.def α β γ) ▸ h.compIsFun (compFunFunFun' α (β ⟶ γ) γ)
                                                  (compFunFun' (appFunFun' β γ) (α ⟶ γ))
 
-  def swapFunFunFun' (α β γ : V) : (α ⟶ β ⟶ γ) ⟶' (β ⟶ α ⟶ γ) := HasFun.mkFun' (swapFunFunIsFun α β γ)
-  def swapFunFunFun  (α β γ : V) : (α ⟶ β ⟶ γ) ⟶  (β ⟶ α ⟶ γ) := HasFun.mkFun  (swapFunFunIsFun α β γ)
+  def swapFunFunFun' (α β γ : U) : (α ⟶ β ⟶ γ) ⟶' (β ⟶ α ⟶ γ) := HasInternalFunctors.mkFun' (swapFunFunIsFun α β γ)
+  def swapFunFunFun  (α β γ : U) : (α ⟶ β ⟶ γ) ⟶  (β ⟶ α ⟶ γ) := HasInternalFunctors.mkFun  (swapFunFunIsFun α β γ)
 
-  @[simp] theorem swapFunFunFun.eff (α β γ : V) (F : α ⟶ β ⟶ γ) :
-    (swapFunFunFun α β γ) F = swapFunFun F :=
-  by apply HasFun.mkFun.eff
+  @[simp] theorem swapFunFunFun.eff (α β γ : U) (F : α ⟶ β ⟶ γ) :
+    (swapFunFunFun α β γ)⟮F⟯ = swapFunFun F :=
+  by apply HasInternalFunctors.mkFun.eff
 
   -- In particular, reverse composition is also functorial.
 
-  theorem revCompFunFun.def (α : V) {β γ : V} (G : β ⟶' γ) (F : α ⟶ β) :
-    HasFun.mkFun (h.compIsFun (HasFun.toBundled F) G) = (compFunFun F γ) (HasFun.fromBundled G) :=
-  Eq.subst (motive := λ H => HasFun.mkFun (h.compIsFun (HasFun.toBundled F) H) = (compFunFun F γ) (HasFun.fromBundled G))
-           (HasFun.toFromBundled G)
-           (Eq.symm (compFunFun.eff F γ (HasFun.fromBundled G)))
+  theorem revCompFunFun.def (α : U) {β γ : U} (G : β ⟶' γ) (F : α ⟶ β) :
+    HasInternalFunctors.mkFun (h.compIsFun (HasInternalFunctors.toBundled F) G) = (compFunFun F γ)⟮HasInternalFunctors.fromBundled G⟯ :=
+  Eq.subst (motive := λ H => HasInternalFunctors.mkFun (h.compIsFun (HasInternalFunctors.toBundled F) H) = (compFunFun F γ)⟮HasInternalFunctors.fromBundled G⟯)
+           (HasInternalFunctors.toFromBundled G)
+           (Eq.symm (compFunFun.eff F γ (HasInternalFunctors.fromBundled G)))
 
-  def revCompFunIsFun (α : V) {β γ : V} (G : β ⟶' γ) :
-    HasIsFun.IsFun (λ F : α ⟶ β => HasFun.mkFun (h.compIsFun (HasFun.toBundled F) G)) :=
-  funext (revCompFunFun.def α G) ▸ swapIsFun (compFunFunFun' α β γ) (HasFun.fromBundled G)
+  def revCompFunIsFun (α : U) {β γ : U} (G : β ⟶' γ) :
+    HasExternalFunctors.IsFun (λ F : α ⟶ β => HasInternalFunctors.mkFun (h.compIsFun (HasInternalFunctors.toBundled F) G)) :=
+  funext (revCompFunFun.def α G) ▸ swapIsFun (compFunFunFun' α β γ) (HasInternalFunctors.fromBundled G)
 
-  def revCompFunFun' (α : V) {β γ : V} (G : β ⟶' γ) : (α ⟶ β) ⟶' (α ⟶ γ) := HasFun.mkFun' (revCompFunIsFun α G)
-  def revCompFunFun  (α : V) {β γ : V} (G : β ⟶  γ) : (α ⟶ β) ⟶  (α ⟶ γ) := HasFun.mkFun  (revCompFunIsFun α (HasFun.toBundled G))
+  def revCompFunFun' (α : U) {β γ : U} (G : β ⟶' γ) : (α ⟶ β) ⟶' (α ⟶ γ) := HasInternalFunctors.mkFun' (revCompFunIsFun α G)
+  def revCompFunFun  (α : U) {β γ : U} (G : β ⟶  γ) : (α ⟶ β) ⟶  (α ⟶ γ) := HasInternalFunctors.mkFun  (revCompFunIsFun α (HasInternalFunctors.toBundled G))
 
-  @[simp] theorem revCompFunFun.eff (α : V) {β γ : V} (G : β ⟶ γ) (F : α ⟶ β) :
-    (revCompFunFun α G) F = G ⊙ F :=
-  by apply HasFun.mkFun.eff
+  @[simp] theorem revCompFunFun.eff (α : U) {β γ : U} (G : β ⟶ γ) (F : α ⟶ β) :
+    (revCompFunFun α G)⟮F⟯ = G ⊙ F :=
+  by apply HasInternalFunctors.mkFun.eff
 
-  theorem revCompFunFunFun.def (α β γ : V) (G : β ⟶ γ) :
-    HasFun.mkFun (revCompFunIsFun α (HasFun.toBundled G)) = HasFun.mkFun (swapIsFun (compFunFunFun' α β γ) G) :=
-  congrArg (λ H => HasFun.mkFun (swapIsFun (compFunFunFun' α β γ) H)) (HasFun.fromToBundled G) ▸ elimRec
+  theorem revCompFunFunFun.def (α β γ : U) (G : β ⟶ γ) :
+    HasInternalFunctors.mkFun (revCompFunIsFun α (HasInternalFunctors.toBundled G)) = HasInternalFunctors.mkFun (swapIsFun (compFunFunFun' α β γ) G) :=
+  congrArg (λ H => HasInternalFunctors.mkFun (swapIsFun (compFunFunFun' α β γ) H)) (HasInternalFunctors.fromToBundled G) ▸ elimRec
 
-  def revCompFunFunIsFun (α β γ : V) :
-    HasIsFun.IsFun (λ G : β ⟶ γ => revCompFunFun α G) :=
+  def revCompFunFunIsFun (α β γ : U) :
+    HasExternalFunctors.IsFun (λ G : β ⟶ γ => revCompFunFun α G) :=
   funext (revCompFunFunFun.def α β γ) ▸ swapFunIsFun (compFunFunFun' α β γ)
 
-  def revCompFunFunFun' (α β γ : V) : (β ⟶ γ) ⟶' (α ⟶ β) ⟶ (α ⟶ γ) := HasFun.mkFun' (revCompFunFunIsFun α β γ)
-  def revCompFunFunFun  (α β γ : V) : (β ⟶ γ) ⟶  (α ⟶ β) ⟶ (α ⟶ γ) := HasFun.mkFun  (revCompFunFunIsFun α β γ)
+  def revCompFunFunFun' (α β γ : U) : (β ⟶ γ) ⟶' (α ⟶ β) ⟶ (α ⟶ γ) := HasInternalFunctors.mkFun' (revCompFunFunIsFun α β γ)
+  def revCompFunFunFun  (α β γ : U) : (β ⟶ γ) ⟶  (α ⟶ β) ⟶ (α ⟶ γ) := HasInternalFunctors.mkFun  (revCompFunFunIsFun α β γ)
 
-  @[simp] theorem revCompFunFunFun.eff (α β γ : V) (G : β ⟶ γ) :
-    (revCompFunFunFun α β γ) G = revCompFunFun α G :=
-  by apply HasFun.mkFun.eff
+  @[simp] theorem revCompFunFunFun.eff (α β γ : U) (G : β ⟶ γ) :
+    (revCompFunFunFun α β γ)⟮G⟯ = revCompFunFun α G :=
+  by apply HasInternalFunctors.mkFun.eff
 
   -- Composition of a function with two arguments.
 
-  def compFun₂ {α β γ δ : V} (F : α ⟶ β ⟶ γ) (G : γ ⟶ δ) : α ⟶ β ⟶ δ := swapFunFun (revCompFunFun α G ⊙ swapFunFun F)
+  def compFun₂ {α β γ δ : U} (F : α ⟶ β ⟶ γ) (G : γ ⟶ δ) : α ⟶ β ⟶ δ := swapFunFun (revCompFunFun α G ⊙ swapFunFun F)
 
   -- The S combinator (see https://en.wikipedia.org/wiki/SKI_combinator_calculus), which in our case says
   -- that if we can functorially construct a functor `H : β ⟶ γ` and an argument `b : β`, then the
   -- construction of `H b` is also functorial.
 
-  theorem substFun.def {α β γ : V} (F : α ⟶' β ⟶ γ) (G : α ⟶' β) (a : α) :
-    F a (G a) = HasFun.mkFun (swapIsFun F (G a)) a :=
-  Eq.symm (HasFun.mkFun.eff (swapIsFun F (G a)) a)
+  theorem substFun.def {α β γ : U} (F : α ⟶' β ⟶ γ) (G : α ⟶' β) (a : α) :
+    F a (G a) = HasInternalFunctors.mkFun (swapIsFun F (G a)) a :=
+  Eq.symm (HasInternalFunctors.mkFun.eff (swapIsFun F (G a)) a)
 
-  def substIsFun {α β γ : V} (F : α ⟶' β ⟶ γ) (G : α ⟶' β) : HasIsFun.IsFun (λ a : α => F a (G a)) :=
+  def substIsFun {α β γ : U} (F : α ⟶' β ⟶ γ) (G : α ⟶' β) : HasExternalFunctors.IsFun (λ a : α => F a (G a)) :=
   funext (substFun.def F G) ▸ h.dupIsFun (swapFunFun' F ⊙' G)
 
-  def substFun' {α β γ : V} (F : α ⟶' β ⟶ γ) (G : α ⟶' β) : α ⟶' γ := HasFun.mkFun' (substIsFun F                    G)
-  def substFun  {α β γ : V} (F : α ⟶  β ⟶ γ) (G : α ⟶  β) : α ⟶  γ := HasFun.mkFun  (substIsFun (HasFun.toBundled F) (HasFun.toBundled G))
+  def substFun' {α β γ : U} (F : α ⟶' β ⟶ γ) (G : α ⟶' β) : α ⟶' γ := HasInternalFunctors.mkFun' (substIsFun F                    G)
+  def substFun  {α β γ : U} (F : α ⟶  β ⟶ γ) (G : α ⟶  β) : α ⟶  γ := HasInternalFunctors.mkFun  (substIsFun (HasInternalFunctors.toBundled F) (HasInternalFunctors.toBundled G))
 
-  @[simp] theorem substFun.eff {α β γ : V} (F : α ⟶ β ⟶ γ) (G : α ⟶ β) (a : α) :
-    (substFun F G) a = F a (G a) :=
-  by apply HasFun.mkFun.eff
+  @[simp] theorem substFun.eff {α β γ : U} (F : α ⟶ β ⟶ γ) (G : α ⟶ β) (a : α) :
+    (substFun F G) a = F⟮a⟯ (G a) :=
+  by apply HasInternalFunctors.mkFun.eff
 
-  theorem substFunFun.def {α β γ : V} (F : α ⟶' β ⟶ γ) (G : α ⟶ β) :
-    HasFun.mkFun (substIsFun F (HasFun.toBundled G)) =
-    HasFun.mkFun (h.dupIsFun (HasFun.toBundled (HasFun.mkFun (h.compIsFun (HasFun.toBundled G) (swapFunFun' F))))) :=
-  HasFun.toFromBundled _ ▸ elimRec
+  theorem substFunFun.def {α β γ : U} (F : α ⟶' β ⟶ γ) (G : α ⟶ β) :
+    HasInternalFunctors.mkFun (substIsFun F (HasInternalFunctors.toBundled G)) =
+    HasInternalFunctors.mkFun (h.dupIsFun (HasInternalFunctors.toBundled (HasInternalFunctors.mkFun (h.compIsFun (HasInternalFunctors.toBundled G) (swapFunFun' F))))) :=
+  HasInternalFunctors.toFromBundled _ ▸ elimRec
 
-  def substFunIsFun {α β γ : V} (F : α ⟶' β ⟶ γ) :
-    HasIsFun.IsFun (λ G : α ⟶ β => HasFun.mkFun (substIsFun F (HasFun.toBundled G))) :=
+  def substFunIsFun {α β γ : U} (F : α ⟶' β ⟶ γ) :
+    HasExternalFunctors.IsFun (λ G : α ⟶ β => HasInternalFunctors.mkFun (substIsFun F (HasInternalFunctors.toBundled G))) :=
   funext (substFunFun.def F) ▸ h.compIsFun (revCompFunFun' α (swapFunFun' F)) (dupFunFun' α γ)
 
-  def substFunFun' {α β γ : V} (F : α ⟶' β ⟶ γ) : (α ⟶ β) ⟶' (α ⟶ γ) := HasFun.mkFun' (substFunIsFun F)
-  def substFunFun  {α β γ : V} (F : α ⟶  β ⟶ γ) : (α ⟶ β) ⟶  (α ⟶ γ) := HasFun.mkFun  (substFunIsFun (HasFun.toBundled F))
+  def substFunFun' {α β γ : U} (F : α ⟶' β ⟶ γ) : (α ⟶ β) ⟶' (α ⟶ γ) := HasInternalFunctors.mkFun' (substFunIsFun F)
+  def substFunFun  {α β γ : U} (F : α ⟶  β ⟶ γ) : (α ⟶ β) ⟶  (α ⟶ γ) := HasInternalFunctors.mkFun  (substFunIsFun (HasInternalFunctors.toBundled F))
 
-  @[simp] theorem substFunFun.eff {α β γ : V} (F : α ⟶ β ⟶ γ) (G : α ⟶ β) :
-    (substFunFun F) G = substFun F G :=
-  by apply HasFun.mkFun.eff
+  @[simp] theorem substFunFun.eff {α β γ : U} (F : α ⟶ β ⟶ γ) (G : α ⟶ β) :
+    (substFunFun F)⟮G⟯ = substFun F G :=
+  by apply HasInternalFunctors.mkFun.eff
 
-  theorem substFunFunFun.def (α β γ : V) (F : α ⟶ β ⟶ γ) :
-    substFunFun F = HasFun.mkFun (h.compIsFun (HasFun.toBundled (revCompFunFun α (swapFunFun F))) (dupFunFun' α γ)) :=
-  HasFun.toFromBundled _ ▸ HasFun.toFromBundled _ ▸ elimRec
+  theorem substFunFunFun.def (α β γ : U) (F : α ⟶ β ⟶ γ) :
+    substFunFun F = HasInternalFunctors.mkFun (h.compIsFun (HasInternalFunctors.toBundled (revCompFunFun α (swapFunFun F))) (dupFunFun' α γ)) :=
+  HasInternalFunctors.toFromBundled _ ▸ HasInternalFunctors.toFromBundled _ ▸ elimRec
 
-  def substFunFunIsFun (α β γ : V) : HasIsFun.IsFun (λ F : α ⟶ β ⟶ γ => substFunFun F) :=
+  def substFunFunIsFun (α β γ : U) : HasExternalFunctors.IsFun (λ F : α ⟶ β ⟶ γ => substFunFun F) :=
   funext (substFunFunFun.def α β γ) ▸ h.compIsFun (revCompFunFunFun' α β (α ⟶ γ) ⊙' swapFunFunFun' α β γ)
                                                   (revCompFunFun' (α ⟶ β) (dupFunFun' α γ))
 
-  def substFunFunFun' (α β γ : V) : (α ⟶ β ⟶ γ) ⟶' (α ⟶ β) ⟶ (α ⟶ γ) := HasFun.mkFun' (substFunFunIsFun α β γ)
-  def substFunFunFun  (α β γ : V) : (α ⟶ β ⟶ γ) ⟶  (α ⟶ β) ⟶ (α ⟶ γ) := HasFun.mkFun  (substFunFunIsFun α β γ)
+  def substFunFunFun' (α β γ : U) : (α ⟶ β ⟶ γ) ⟶' (α ⟶ β) ⟶ (α ⟶ γ) := HasInternalFunctors.mkFun' (substFunFunIsFun α β γ)
+  def substFunFunFun  (α β γ : U) : (α ⟶ β ⟶ γ) ⟶  (α ⟶ β) ⟶ (α ⟶ γ) := HasInternalFunctors.mkFun  (substFunFunIsFun α β γ)
 
-  @[simp] theorem substFunFunFun.eff (α β γ : V) (F : α ⟶ β ⟶ γ) :
-    (substFunFunFun α β γ) F = substFunFun F :=
-  by apply HasFun.mkFun.eff
+  @[simp] theorem substFunFunFun.eff (α β γ : U) (F : α ⟶ β ⟶ γ) :
+    (substFunFunFun α β γ)⟮F⟯ = substFunFun F :=
+  by apply HasInternalFunctors.mkFun.eff
 
 
 
   -- Using the functoriality axioms and the constructions above, we can algorithmically prove
-  -- functoriality of lambda terms. The algorithm to prove `HasIsFun.IsFun (λ a : α => t)` is as follows:
+  -- functoriality of lambda terms. The algorithm to prove `HasExternalFunctors.IsFun (λ a : α => t)` is as follows:
   --
   --  Case                                 | Proof
   -- --------------------------------------+--------------------------------------------------------------
@@ -171,7 +173,7 @@ namespace HasFunOp
   --  `t` is `G b` with `G : β ⟶ γ`:       |
   --    `a` appears only in `b`            | Prove that `λ a => b` is functorial, yielding a functor
   --                                       | `F : α ⟶ β`. Then the proof is `compIsFun F G`.
-  --      `b` is `a`                       | Optimization: `HasFun.isFun G`
+  --      `b` is `a`                       | Optimization: `HasInternalFunctors.isFun G`
   --    `a` appears only in `G`            | Prove that `λ a => G` is functorial, yielding a functor
   --                                       | `F : α ⟶ β ⟶ γ`. Then the proof is `swapIsFun F b`.
   --      `G` is `a`                       | Optimization: `appIsFun b γ`
@@ -179,12 +181,23 @@ namespace HasFunOp
   --                                       | `F₁ : α ⟶ β ⟶ γ`. Prove that `λ a => b` is functorial,
   --                                       | yielding a functor `F₂ : α ⟶ β`. Then the proof is
   --                                       | `substIsFun F₁ F₂`.
-  --  `t` is `HasFun.mkFun (λ b : β => c)` | Prove that `λ a => c` is functorial when regarding `b` as a
+  --  `t` is `HasInternalFunctors.mkFun (λ b : β => c)` | Prove that `λ a => c` is functorial when regarding `b` as a
   --                                       | constant, yielding a functor `F : α ⟶ γ` for every `b`.
   --                                       | Prove that  `λ b => F` is functorial, yielding a functor
   --                                       | `G : β ⟶ α ⟶ γ`. Then the proof is `swapFunIsFun G`.
   --
   -- (This list does not contain all possible optimizations.)
+
+
+
+-- TODO: Add equivalences.
+-- TODO: Add morphisms.
+
+  instance : HasRefl    h.Fun := ⟨idFun⟩
+  instance : HasTrans   h.Fun := ⟨compFunFunFun _ _ _⟩
+  instance : IsPreorder h.Fun := ⟨⟩
+
+  instance hasArrows : HasArrows ⌈U⌉ U := ⟨h.Fun⟩
 
 end HasFunOp
 
@@ -192,11 +205,11 @@ end HasFunOp
 
 namespace GeneralizedProperty
 
-  def ConstProp (α : Sort u) {V : Sort v} [s : HasInstances V] {β : V} (c : β) : GeneralizedProperty α V := λ _ => β
+  def ConstProp (α : Sort u) {V : Universe} {β : V} (c : β) : GeneralizedProperty α V := λ _ => β
 
   namespace ConstProp
 
-    variable (α : Sort u) {V : Sort v} [s : HasInstances V] {β : V} (c : β)
+    variable (α : Sort u) {V : Universe} {β : V} (c : β)
 
     instance hasInst : HasInst (ConstProp α c) := ⟨λ _ => c⟩
 
@@ -208,13 +221,16 @@ end GeneralizedProperty
 
 namespace GeneralizedRelation
 
-  def ConstRel (α : Sort u) {V : Sort v} [s : IsKind V] {β : V} (c : β) : GeneralizedRelation α V := λ _ _ => β
+  def ConstRel (α : Sort u) {V : Universe} {β : V} (c : β) : GeneralizedRelation α V := λ _ _ => β
 
   namespace ConstRel
   
-    variable (α : Sort u) {V : Sort v} [s : IsKind V] {β : V} (c : β)
+    variable (α : Sort u) {V : Universe} {β : V} (c : β)
 
     instance hasRefl  : HasRefl  (ConstRel α c) := ⟨λ _ => c⟩
+
+    variable [HasFunOp V]
+
     instance hasSymm  : HasSymm  (ConstRel α c) := ⟨HasFunOp.idFun β⟩
     instance hasTrans : HasTrans (ConstRel α c) := ⟨HasFunOp.constFun β (HasFunOp.idFun β)⟩
 
@@ -224,12 +240,12 @@ namespace GeneralizedRelation
     @[simp] theorem symmEq  {a₁ a₂    : α} : (hasSymm  α c).symm'  (a := a₁) (b := a₂)           c   = c :=
     HasFunOp.idFun.eff β c
     @[simp] theorem transEq {a₁ a₂ a₃ : α} : (hasTrans α c).trans' (a := a₁) (b := a₂) (c := a₃) c c = c :=
-    let h₁ := congrArg HasFun.funCoe (HasFunOp.constFun.eff β (HasFunOp.idFun β) c);
+    let h₁ := congrArg HasInternalFunctors.funCoe (HasFunOp.constFun.eff β (HasFunOp.idFun β) c);
     Eq.trans (congrFun h₁ c) (HasFunOp.idFun.eff β c)
 
   end ConstRel
 
-  variable {α : Sort u} {V : Sort v} [s : IsKind V]
+  variable {α : Sort u} {V : Universe} [HasFunOp V]
 
   def HasTrans.revTrans   {R : GeneralizedRelation α V} [h : HasTrans R] {a b c : α} : R b c ⟶ R a b ⟶ R a c := HasFunOp.swapFunFun h.trans
   def HasTrans.revTrans'' {R : GeneralizedRelation α V} [h : HasTrans R] {a b c : α} (g : R b c) : R a b ⟶ R a c := HasFunOp.swapFun h.trans g
@@ -240,117 +256,102 @@ open GeneralizedRelation
 
 
 
--- TODO: Add equivalences.
--- TODO: Add morphisms.
+namespace HasFunctorialArrows
 
-namespace IsKind
+  variable (U : Universe) [HasInternalFunctors U] [h : HasFunctorialArrows U]
 
-  variable (V : Sort v) [s : IsKind V]
+  def arrowCongrArg  {α β : U} (F : α ⟶{U} β) {a b : α} : (a ⇝ b) ⟶{h.arrowUniverse} (F a ⇝ F b) := h.arrowCongr⟮HasRefl.refl F⟯
+  def arrowCongrArg' {α β : U} (F : α ⟶'   β) {a b : α} : (a ⇝ b) ⟶{h.arrowUniverse} (F a ⇝ F b) := HasInternalFunctors.fromBundled.coe F ▸ arrowCongrArg U (HasInternalFunctors.fromBundled F)
 
-  instance : HasRefl    s.Fun := ⟨HasFunOp.idFun⟩
-  instance : HasTrans   s.Fun := ⟨HasFunOp.compFunFunFun _ _ _⟩
-  instance : IsPreorder s.Fun := ⟨⟩
+  def arrowCongrFun {α β : U} {F G : α ⟶{U} β} (a : α) : (F ⇝ G) ⟶{h.arrowUniverse} (F a ⇝ G a) := HasFunOp.swapFun h.arrowCongr (HasRefl.refl a)
 
-  instance hasArrows : HasArrows V V := ⟨s.Fun⟩
+end HasFunctorialArrows
 
-end IsKind
+namespace HasFunctorialEquivalences
 
+  variable (U : Universe) [HasInternalFunctors U] [h : HasFunctorialEquivalences U]
 
+  def equivCongrArg  {α β : U} (F : α ⟶{U} β) {a b : α} : a ≃ b ⟶{h.equivUniverse} F a ≃ F b := h.equivCongr⟮HasRefl.refl F⟯
+  def equivCongrArg' {α β : U} (F : α ⟶'   β) {a b : α} : a ≃ b ⟶{h.equivUniverse} F a ≃ F b := HasInternalFunctors.fromBundled.coe F ▸ equivCongrArg U (HasInternalFunctors.fromBundled F)
 
-namespace HasInstanceArrows
+  def equivCongrFun {α β : U} {F G : α ⟶{U} β} (a : α) : F ≃ G ⟶{h.equivUniverse} F a ≃ G a := HasFunOp.swapFun h.equivCongr (HasRefl.refl a)
 
-  variable (V : Sort v) [IsKind V] [HasInstanceArrows V]
-
-  def arrCongrArg  {α β : V} (F : α ⟶{V} β) {a b : α} : (a ⇝ b) ⟶ (F a ⇝ F b) := (HasFun.funCoe (arrCongr V)) (HasRefl.refl F)
-  def arrCongrArg' {α β : V} (F : α ⟶'   β) {a b : α} : (a ⇝ b) ⟶ (F a ⇝ F b) := HasFun.fromBundled.coe F ▸ arrCongrArg V (HasFun.fromBundled F)
-
-  def arrCongrFun {α β : V} {F G : α ⟶{V} β} (a : α) : (F ⇝ G) ⟶ (F a ⇝ G a) := HasFunOp.swapFun (arrCongr V) (HasRefl.refl a)
-
-end HasInstanceArrows
-
-namespace HasInstanceEquivalences
-
-  variable (V : Sort v) [IsKind V] [HasInstanceEquivalences V]
-
-  def funCongrArg  {α β : V} (F : α ⟶{V} β) {a b : α} : a ≃ b ⟶ F a ≃ F b := (HasFun.funCoe (funCongr V)) (HasRefl.refl F)
-  def funCongrArg' {α β : V} (F : α ⟶'   β) {a b : α} : a ≃ b ⟶ F a ≃ F b := HasFun.fromBundled.coe F ▸ funCongrArg V (HasFun.fromBundled F)
-
-  def funCongrFun {α β : V} {F G : α ⟶{V} β} (a : α) : F ≃ G ⟶ F a ≃ G a := HasFunOp.swapFun (funCongr V) (HasRefl.refl a)
-
-end HasInstanceEquivalences
+end HasFunctorialEquivalences
 
 
 
 -- TODO: Should we use actual abstract equivalence here?
 
-structure Iff' {V : Sort v} [IsKind V] (α β : V) where
+structure Iff' {U : Universe} [HasInternalFunctors U] (α β : U) where
 (mp  : α ⟶ β)
 (mpr : β ⟶ α)
 
-notation:20 α:21 " ⟷{" W:0 "} " β:21 => Iff' (V := W) α β
+notation:20 α:21 " ⟷{" U':0 "} " β:21 => Iff' (U := U') α β
 
 
 
 section Morphisms
 
-  variable {α : Sort u} (V : Sort v) [IsKind V] [he : HasInstanceEquivalences V] {R : GeneralizedRelation α V}
+  variable {α : Sort u} {U : Universe} [HasInternalFunctors U] [he : HasFunctorialEquivalences U] {R : GeneralizedRelation α U}
+
+  instance : HasFunctorialArrows U := HasFunctorialEquivalences.toHasFunctorialArrows U
 
   open IsCompositionRelation
 
   namespace IsCompositionRelation
 
-    variable [h : IsCompositionRelation R]
+    variable [HasTrans R] [IsCompositionRelation R]
 
-    def comp_congrArg {a b c : α} {f₁ f₂ : R a b} {g₁ g₂ : R b c} : f₁ ≃ f₂ ⟶ g₁ ≃ g₂ ⟶ g₁ • f₁ ≃ g₂ • f₂ :=
-    HasInstanceEquivalences.funCongr V ⊙ HasInstanceEquivalences.funCongrArg V HasTrans.trans
+    def comp_congrArg {a b c : α} {f₁ f₂ : R a b} {g₁ g₂ : R b c} : f₁ ≃ f₂ ⟶{he.equivUniverse} g₁ ≃ g₂ ⟶ g₁ • f₁ ≃ g₂ • f₂ :=
+    he.equivCongr ⊙ HasFunctorialEquivalences.equivCongrArg U HasTrans.trans
 
-    def comp_congrArg_left  {a b c : α} {f : R a b} {g₁ g₂ : R b c} : g₁ ≃ g₂ ⟶ g₁ • f ≃ g₂ • f :=
-    HasInstanceEquivalences.funCongrArg V (HasTrans.trans'' f)
+    def comp_congrArg_left  {a b c : α} {f : R a b} {g₁ g₂ : R b c} : g₁ ≃ g₂ ⟶{he.equivUniverse} g₁ • f ≃ g₂ • f :=
+    HasFunctorialEquivalences.equivCongrArg U (HasTrans.trans'' f)
 
-    def comp_congrArg_right {a b c : α} {f₁ f₂ : R a b} {g : R b c} : f₁ ≃ f₂ ⟶ g • f₁ ≃ g • f₂ :=
-    HasFunOp.swapFun (comp_congrArg V) (HasRefl.refl g)
+    def comp_congrArg_right {a b c : α} {f₁ f₂ : R a b} {g : R b c} : f₁ ≃ f₂ ⟶{he.equivUniverse} g • f₁ ≃ g • f₂ :=
+    HasFunOp.swapFun comp_congrArg (HasRefl.refl g)
 
-    def comp_subst  {a b c : α} {f₁ f₂ : R a b} {g₁ g₂ : R b c} {e : R a c} : f₁ ≃ f₂ ⟶ g₁ ≃ g₂ ⟶ g₂ • f₂ ≃ e ⟶ g₁ • f₁ ≃ e :=
-    HasFunOp.compFun₂ (comp_congrArg V) HasTrans.trans
-    def comp_subst' {a b c : α} {f₁ f₂ : R a b} {g₁ g₂ : R b c} {e : R a c} : f₁ ≃ f₂ ⟶ g₁ ≃ g₂ ⟶ e ≃ g₁ • f₁ ⟶ e ≃ g₂ • f₂ :=
-    HasFunOp.compFun₂ (comp_congrArg V) HasTrans.revTrans
+    def comp_subst  {a b c : α} {f₁ f₂ : R a b} {g₁ g₂ : R b c} {e : R a c} : f₁ ≃ f₂ ⟶{he.equivUniverse} g₁ ≃ g₂ ⟶ g₂ • f₂ ≃ e ⟶ g₁ • f₁ ≃ e :=
+    HasFunOp.compFun₂ comp_congrArg HasTrans.trans
+    def comp_subst' {a b c : α} {f₁ f₂ : R a b} {g₁ g₂ : R b c} {e : R a c} : f₁ ≃ f₂ ⟶{he.equivUniverse} g₁ ≃ g₂ ⟶ e ≃ g₁ • f₁ ⟶ e ≃ g₂ • f₂ :=
+    HasFunOp.compFun₂ comp_congrArg HasTrans.revTrans
 
-    def comp_subst_left   {a b c : α} (f : R a b) {g₁ g₂ : R b c} {e : R a c} : g₁ ≃ g₂ ⟶ g₂ • f ≃ e ⟶ g₁ • f ≃ e :=
-    HasTrans.trans    ⊙ comp_congrArg_left V
-    def comp_subst_left'  {a b c : α} (f : R a b) {g₁ g₂ : R b c} {e : R a c} : g₁ ≃ g₂ ⟶ e ≃ g₁ • f ⟶ e ≃ g₂ • f :=
-    HasTrans.revTrans ⊙ comp_congrArg_left V
+    def comp_subst_left   {a b c : α} (f : R a b) {g₁ g₂ : R b c} {e : R a c} : g₁ ≃ g₂ ⟶{he.equivUniverse} g₂ • f ≃ e ⟶ g₁ • f ≃ e :=
+    HasTrans.trans    ⊙ comp_congrArg_left
+    def comp_subst_left'  {a b c : α} (f : R a b) {g₁ g₂ : R b c} {e : R a c} : g₁ ≃ g₂ ⟶{he.equivUniverse} e ≃ g₁ • f ⟶ e ≃ g₂ • f :=
+    HasTrans.revTrans ⊙ comp_congrArg_left
 
-    def comp_subst_right  {a b c : α} {f₁ f₂ : R a b} (g : R b c) {e : R a c} : f₁ ≃ f₂ ⟶ g • f₂ ≃ e ⟶ g • f₁ ≃ e :=
-    HasTrans.trans    ⊙ comp_congrArg_right V
-    def comp_subst_right' {a b c : α} {f₁ f₂ : R a b} (g : R b c) {e : R a c} : f₁ ≃ f₂ ⟶ e ≃ g • f₁ ⟶ e ≃ g • f₂ :=
-    HasTrans.revTrans ⊙ comp_congrArg_right V
+    def comp_subst_right  {a b c : α} {f₁ f₂ : R a b} (g : R b c) {e : R a c} : f₁ ≃ f₂ ⟶{he.equivUniverse} g • f₂ ≃ e ⟶ g • f₁ ≃ e :=
+    HasTrans.trans    ⊙ comp_congrArg_right
+    def comp_subst_right' {a b c : α} {f₁ f₂ : R a b} (g : R b c) {e : R a c} : f₁ ≃ f₂ ⟶{he.equivUniverse} e ≃ g • f₁ ⟶ e ≃ g • f₂ :=
+    HasTrans.revTrans ⊙ comp_congrArg_right
 
-    def applyAssocLR_left  {a b c d : α} {f : R a b} {g : R b c} {h : R c d} {e : R a d} : (h • g) • f ≃ e ⟶ h • (g • f) ≃ e :=
+    def applyAssocLR_left  {a b c d : α} {f : R a b} {g : R b c} {h : R c d} {e : R a d} : (h • g) • f ≃ e ⟶{he.equivUniverse} h • (g • f) ≃ e :=
     HasTrans.trans'' (assocRL f g h)
-    def applyAssocRL_left  {a b c d : α} {f : R a b} {g : R b c} {h : R c d} {e : R a d} : h • (g • f) ≃ e ⟶ (h • g) • f ≃ e :=
+    def applyAssocRL_left  {a b c d : α} {f : R a b} {g : R b c} {h : R c d} {e : R a d} : h • (g • f) ≃ e ⟶{he.equivUniverse} (h • g) • f ≃ e :=
     HasTrans.trans'' (assocLR f g h)
-    def applyAssocLR_right {a b c d : α} {f : R a b} {g : R b c} {h : R c d} {e : R a d} : e ≃ (h • g) • f ⟶ e ≃ h • (g • f) :=
+    def applyAssocLR_right {a b c d : α} {f : R a b} {g : R b c} {h : R c d} {e : R a d} : e ≃ (h • g) • f ⟶{he.equivUniverse} e ≃ h • (g • f) :=
     HasTrans.revTrans'' (assocLR f g h)
-    def applyAssocRL_right {a b c d : α} {f : R a b} {g : R b c} {h : R c d} {e : R a d} : e ≃ h • (g • f) ⟶ e ≃ (h • g) • f :=
+    def applyAssocRL_right {a b c d : α} {f : R a b} {g : R b c} {h : R c d} {e : R a d} : e ≃ h • (g • f) ⟶{he.equivUniverse} e ≃ (h • g) • f :=
     HasTrans.revTrans'' (assocRL f g h)
 
     def applyAssocLR {a β₁ β₂ γ₁ γ₂ d : α} {f₁ : R a β₁} {f₂ : R a β₂} {g₁ : R β₁ γ₁} {g₂ : R β₂ γ₂} {h₁ : R γ₁ d} {h₂ : R γ₂ d} :
-      (h₁ • g₁) • f₁ ≃ (h₂ • g₂) • f₂ ⟶ h₁ • (g₁ • f₁) ≃ h₂ • (g₂ • f₂) :=
-    applyAssocLR_right V ⊙ applyAssocLR_left V
+      (h₁ • g₁) • f₁ ≃ (h₂ • g₂) • f₂ ⟶{he.equivUniverse} h₁ • (g₁ • f₁) ≃ h₂ • (g₂ • f₂) :=
+    applyAssocLR_right ⊙ applyAssocLR_left
     def applyAssocRL {a β₁ β₂ γ₁ γ₂ d : α} {f₁ : R a β₁} {f₂ : R a β₂} {g₁ : R β₁ γ₁} {g₂ : R β₂ γ₂} {h₁ : R γ₁ d} {h₂ : R γ₂ d} :
-      h₁ • (g₁ • f₁) ≃ h₂ • (g₂ • f₂) ⟶ (h₁ • g₁) • f₁ ≃ (h₂ • g₂) • f₂ :=
-    applyAssocRL_right V ⊙ applyAssocRL_left V
+      h₁ • (g₁ • f₁) ≃ h₂ • (g₂ • f₂) ⟶{he.equivUniverse} (h₁ • g₁) • f₁ ≃ (h₂ • g₂) • f₂ :=
+    applyAssocRL_right ⊙ applyAssocRL_left
 
   end IsCompositionRelation
 
   namespace IsMorphismRelation
 
-    variable [h : IsMorphismRelation R]
+    variable [IsPreorder R] [IsMorphismRelation R]
 
-    def leftCancelId  {a b : α} (f : R a b) {e : R b b} : e ≃ ident R b ⟶ e • f ≃ f :=
-    HasFunOp.swapFun (comp_subst_left  V f) (h.leftId  f)
-    def rightCancelId {a b : α} (f : R a b) {e : R a a} : e ≃ ident R a ⟶ f • e ≃ f :=
-    HasFunOp.swapFun (comp_subst_right V f) (h.rightId f)
+    def leftCancelId  {a b : α} (f : R a b) {e : R b b} : e ≃ ident R b ⟶{he.equivUniverse} e • f ≃ f :=
+    HasFunOp.swapFun (comp_subst_left  f) (leftId  f)
+    def rightCancelId {a b : α} (f : R a b) {e : R a a} : e ≃ ident R a ⟶{he.equivUniverse} f • e ≃ f :=
+    HasFunOp.swapFun (comp_subst_right f) (rightId f)
 
   end IsMorphismRelation
 
@@ -358,67 +359,64 @@ section Morphisms
 
   namespace IsIsomorphismRelation
 
-    variable [IsIsomorphismRelation R]
+    variable [IsEquivalence R] [IsIsomorphismRelation R]
 
-    def inv_congrArg {a b : α} {f₁ f₂ : R a b} : f₁ ≃ f₂ ⟶ f₁⁻¹ ≃ f₂⁻¹ :=
-    HasInstanceEquivalences.funCongrArg V HasSymm.symm
+    def inv_congrArg {a b : α} {f₁ f₂ : R a b} : f₁ ≃ f₂ ⟶{he.equivUniverse} f₁⁻¹ ≃ f₂⁻¹ :=
+    HasFunctorialEquivalences.equivCongrArg U HasSymm.symm
 
-    def inv_subst  {a b : α} {f₁ f₂ : R a b} {e : R b a} : f₁ ≃ f₂ ⟶ f₂⁻¹ ≃ e ⟶ f₁⁻¹ ≃ e :=
-    HasTrans.trans    ⊙ inv_congrArg V
-    def inv_subst' {a b : α} {f₁ f₂ : R a b} {e : R b a} : f₁ ≃ f₂ ⟶ e ≃ f₁⁻¹ ⟶ e ≃ f₂⁻¹ :=
-    HasTrans.revTrans ⊙ inv_congrArg V
+    def inv_subst  {a b : α} {f₁ f₂ : R a b} {e : R b a} : f₁ ≃ f₂ ⟶{he.equivUniverse} f₂⁻¹ ≃ e ⟶ f₁⁻¹ ≃ e :=
+    HasTrans.trans    ⊙ inv_congrArg
+    def inv_subst' {a b : α} {f₁ f₂ : R a b} {e : R b a} : f₁ ≃ f₂ ⟶{he.equivUniverse} e ≃ f₁⁻¹ ⟶ e ≃ f₂⁻¹ :=
+    HasTrans.revTrans ⊙ inv_congrArg
 
-    def leftCancel'     {a b c : α} (f : R a b) (g : R b c) : (g⁻¹ • g) • f ≃ f := leftCancelId  V f (leftInv  g)
-    def leftCancel      {a b c : α} (f : R a b) (g : R b c) : g⁻¹ • (g • f) ≃ f := applyAssocLR_left V (leftCancel'     V f g)
-    def leftCancelInv'  {a b c : α} (f : R a b) (g : R c b) : (g • g⁻¹) • f ≃ f := leftCancelId  V f (rightInv g)
-    def leftCancelInv   {a b c : α} (f : R a b) (g : R c b) : g • (g⁻¹ • f) ≃ f := applyAssocLR_left V (leftCancelInv'  V f g)
-    def rightCancel'    {a b c : α} (f : R a b) (g : R c a) : f • (g • g⁻¹) ≃ f := rightCancelId V f (rightInv g)
-    def rightCancel     {a b c : α} (f : R a b) (g : R c a) : (f • g) • g⁻¹ ≃ f := applyAssocRL_left V (rightCancel'    V f g)
-    def rightCancelInv' {a b c : α} (f : R a b) (g : R a c) : f • (g⁻¹ • g) ≃ f := rightCancelId V f (leftInv  g)
-    def rightCancelInv  {a b c : α} (f : R a b) (g : R a c) : (f • g⁻¹) • g ≃ f := applyAssocRL_left V (rightCancelInv' V f g)
+    def leftCancel'     {a b c : α} (f : R a b) (g : R b c) : (g⁻¹ • g) • f ≃ f := (leftCancelId  f)⟮leftInv  g⟯
+    def leftCancel      {a b c : α} (f : R a b) (g : R b c) : g⁻¹ • (g • f) ≃ f := applyAssocLR_left⟮leftCancel'     f g⟯
+    def leftCancelInv'  {a b c : α} (f : R a b) (g : R c b) : (g • g⁻¹) • f ≃ f := (leftCancelId  f)⟮rightInv g⟯
+    def leftCancelInv   {a b c : α} (f : R a b) (g : R c b) : g • (g⁻¹ • f) ≃ f := applyAssocLR_left⟮leftCancelInv'  f g⟯
+    def rightCancel'    {a b c : α} (f : R a b) (g : R c a) : f • (g • g⁻¹) ≃ f := (rightCancelId f)⟮rightInv g⟯
+    def rightCancel     {a b c : α} (f : R a b) (g : R c a) : (f • g) • g⁻¹ ≃ f := applyAssocRL_left⟮rightCancel'    f g⟯
+    def rightCancelInv' {a b c : α} (f : R a b) (g : R a c) : f • (g⁻¹ • g) ≃ f := (rightCancelId f)⟮leftInv  g⟯
+    def rightCancelInv  {a b c : α} (f : R a b) (g : R a c) : (f • g⁻¹) • g ≃ f := applyAssocRL_left⟮rightCancelInv' f g⟯
 
-    def leftMulInv  {a b c : α} (f₁ : R a b) (f₂ : R a c) (g : R b c) : g • f₁ ≃ f₂ ⟷{he.ArrowKind} f₁ ≃ g⁻¹ • f₂ :=
-    ⟨HasFunOp.swapFun (comp_subst_right' V g⁻¹) ((he.arrowSymm (R a b)).symm' (leftCancel V f₁ g)),
-     HasFunOp.swapFun (comp_subst_right  V g)   (leftCancelInv V f₂ g)⟩
-    def leftMulInv' {a b c : α} (f₁ : R a b) (f₂ : R a c) (g : R c b) : g⁻¹ • f₁ ≃ f₂ ⟷{he.ArrowKind} f₁ ≃ g • f₂ :=
-    ⟨HasFunOp.swapFun (comp_subst_right' V g)   ((he.arrowSymm (R a b)).symm' (leftCancelInv V f₁ g)),
-     HasFunOp.swapFun (comp_subst_right  V g⁻¹) (leftCancel V f₂ g)⟩
+    def leftMulInv  {a b c : α} (f₁ : R a b) (f₂ : R a c) (g : R b c) : g • f₁ ≃ f₂ ⟷{he.equivUniverse} f₁ ≃ g⁻¹ • f₂ :=
+    ⟨HasFunOp.swapFun (comp_subst_right' g⁻¹) (HasSymm.symm' (leftCancel f₁ g)),
+     HasFunOp.swapFun (comp_subst_right  g)   (leftCancelInv f₂ g)⟩
+    def leftMulInv' {a b c : α} (f₁ : R a b) (f₂ : R a c) (g : R c b) : g⁻¹ • f₁ ≃ f₂ ⟷{he.equivUniverse} f₁ ≃ g • f₂ :=
+    ⟨HasFunOp.swapFun (comp_subst_right' g)   (HasSymm.symm' (leftCancelInv f₁ g)),
+     HasFunOp.swapFun (comp_subst_right  g⁻¹) (leftCancel f₂ g)⟩
 
-    def leftMul {a b c : α} (f₁ f₂ : R a b) (g : R b c) : g • f₁ ≃ g • f₂ ⟷{he.ArrowKind} f₁ ≃ f₂ :=
-    ⟨((he.hasArrows (R a b)).isPreorder).revTrans'' (leftCancel V f₂ g) ⊙ (leftMulInv V f₁ (g • f₂) g).mp,
-     comp_congrArg_right V⟩
+    def leftMul {a b c : α} (f₁ f₂ : R a b) (g : R b c) : g • f₁ ≃ g • f₂ ⟷{he.equivUniverse} f₁ ≃ f₂ :=
+    ⟨HasTrans.revTrans'' (leftCancel f₂ g) ⊙ (leftMulInv f₁ (g • f₂) g).mp, comp_congrArg_right⟩
 
-    def rightMulInv  {a b c : α} (f₁ : R a c) (f₂ : R b c) (g : R b a) : f₁ • g ≃ f₂ ⟷{he.ArrowKind} f₁ ≃ f₂ • g⁻¹ :=
-    ⟨HasFunOp.swapFun (comp_subst_left' V g⁻¹) ((he.arrowSymm (R a c)).symm' (rightCancel V f₁ g)),
-     HasFunOp.swapFun (comp_subst_left  V g)   (rightCancelInv V f₂ g)⟩
-    def rightMulInv' {a b c : α} (f₁ : R a c) (f₂ : R b c) (g : R a b) : f₁ • g⁻¹ ≃ f₂ ⟷{he.ArrowKind} f₁ ≃ f₂ • g :=
-    ⟨HasFunOp.swapFun (comp_subst_left' V g)   ((he.arrowSymm (R a c)).symm' (rightCancelInv V f₁ g)),
-     HasFunOp.swapFun (comp_subst_left  V g⁻¹) (rightCancel V f₂ g)⟩
+    def rightMulInv  {a b c : α} (f₁ : R a c) (f₂ : R b c) (g : R b a) : f₁ • g ≃ f₂ ⟷{he.equivUniverse} f₁ ≃ f₂ • g⁻¹ :=
+    ⟨HasFunOp.swapFun (comp_subst_left' g⁻¹) (HasSymm.symm' (rightCancel f₁ g)),
+     HasFunOp.swapFun (comp_subst_left  g)   (rightCancelInv f₂ g)⟩
+    def rightMulInv' {a b c : α} (f₁ : R a c) (f₂ : R b c) (g : R a b) : f₁ • g⁻¹ ≃ f₂ ⟷{he.equivUniverse} f₁ ≃ f₂ • g :=
+    ⟨HasFunOp.swapFun (comp_subst_left' g)   (HasSymm.symm' (rightCancelInv f₁ g)),
+     HasFunOp.swapFun (comp_subst_left  g⁻¹) (rightCancel f₂ g)⟩
 
-    def rightMul {a b c : α} (f₁ f₂ : R a b) (g : R c a) : f₁ • g ≃ f₂ • g ⟷{he.ArrowKind} f₁ ≃ f₂ :=
-    ⟨((he.hasArrows (R a b)).isPreorder).revTrans'' (rightCancel V f₂ g) ⊙ (rightMulInv V f₁ (f₂ • g) g).mp,
-     comp_congrArg_left V⟩
+    def rightMul {a b c : α} (f₁ f₂ : R a b) (g : R c a) : f₁ • g ≃ f₂ • g ⟷{he.equivUniverse} f₁ ≃ f₂ :=
+    ⟨HasTrans.revTrans'' (rightCancel f₂ g) ⊙ (rightMulInv f₁ (f₂ • g) g).mp, comp_congrArg_left⟩
 
-    def eqInvIffInvEq {a b : α} (f : R a b) (g : R b a) : f ≃ g⁻¹ ⟷{he.ArrowKind} f⁻¹ ≃ g :=
-    ⟨HasFunOp.swapFun (inv_subst  V) (invInv g),
-     HasFunOp.swapFun (inv_subst' V) ((he.arrowSymm (R a b)).symm' (invInv f))⟩
+    def eqInvIffInvEq {a b : α} (f : R a b) (g : R b a) : f ≃ g⁻¹ ⟷{he.equivUniverse} f⁻¹ ≃ g :=
+    ⟨HasFunOp.swapFun inv_subst  (invInv g),
+     HasFunOp.swapFun inv_subst' (HasSymm.symm' (invInv f))⟩
 
-    def eqIffEqInv {a b : α} (f₁ f₂ : R a b) : f₁⁻¹ ≃ f₂⁻¹ ⟷{he.ArrowKind} f₁ ≃ f₂ :=
-    ⟨((he.hasArrows (R a b)).isPreorder).revTrans'' (invInv f₂) ⊙ (eqInvIffInvEq V f₁ f₂⁻¹).mpr,
-     inv_congrArg V⟩
+    def eqIffEqInv {a b : α} (f₁ f₂ : R a b) : f₁⁻¹ ≃ f₂⁻¹ ⟷{he.equivUniverse} f₁ ≃ f₂ :=
+    ⟨HasTrans.revTrans'' (invInv f₂) ⊙ (eqInvIffInvEq f₁ f₂⁻¹).mpr, inv_congrArg⟩
 
     def leftRightMul {a b c d : α} (f₁ : R a b) (f₂ : R a c) (g₁ : R b d) (g₂ : R c d) :
-      g₂⁻¹ • g₁ ≃ f₂ • f₁⁻¹ ⟷{he.ArrowKind} g₁ • f₁ ≃ g₂ • f₂ :=
-    ⟨(leftMulInv' V (g₁ • f₁) f₂ g₂).mp ⊙ applyAssocLR_left V ⊙ (rightMulInv V (g₂⁻¹ • g₁) f₂ f₁).mpr,
-     (leftMulInv' V g₁ (f₂ • f₁⁻¹) g₂).mpr ⊙ applyAssocLR_right V ⊙ (rightMulInv V g₁ (g₂ • f₂) f₁).mp⟩
+      g₂⁻¹ • g₁ ≃ f₂ • f₁⁻¹ ⟷{he.equivUniverse} g₁ • f₁ ≃ g₂ • f₂ :=
+    ⟨(leftMulInv' (g₁ • f₁) f₂ g₂).mp ⊙ applyAssocLR_left ⊙ (rightMulInv (g₂⁻¹ • g₁) f₂ f₁).mpr,
+     (leftMulInv' g₁ (f₂ • f₁⁻¹) g₂).mpr ⊙ applyAssocLR_right ⊙ (rightMulInv g₁ (g₂ • f₂) f₁).mp⟩
 
     def swapInv  {a b c d : α} (f₁ : R a b) (f₂ : R c d) (g₁ : R d b) (g₂ : R c a) :
-      g₁⁻¹ • f₁ ≃ f₂ • g₂⁻¹ ⟶ f₁⁻¹ • g₁ ≃ g₂ • f₂⁻¹ :=
-    (leftRightMul V f₂ g₂ g₁ f₁).mpr ⊙ HasSymm.symm ⊙ (leftRightMul V g₂ f₂ f₁ g₁).mp
+      g₁⁻¹ • f₁ ≃ f₂ • g₂⁻¹ ⟶{he.equivUniverse} f₁⁻¹ • g₁ ≃ g₂ • f₂⁻¹ :=
+    (leftRightMul f₂ g₂ g₁ f₁).mpr ⊙ HasSymm.symm ⊙ (leftRightMul g₂ f₂ f₁ g₁).mp
 
     def swapInv' {a b c d : α} (f₁ : R a b) (f₂ : R c d) (g₁ : R d b) (g₂ : R c a) :
-      f₂ • g₂⁻¹ ≃ g₁⁻¹ • f₁ ⟶ g₂ • f₂⁻¹ ≃ f₁⁻¹ • g₁ :=
-    HasSymm.symm ⊙ swapInv V f₁ f₂ g₁ g₂ ⊙ HasSymm.symm
+      f₂ • g₂⁻¹ ≃ g₁⁻¹ • f₁ ⟶{he.equivUniverse} g₂ • f₂⁻¹ ≃ f₁⁻¹ • g₁ :=
+    HasSymm.symm ⊙ swapInv f₁ f₂ g₁ g₂ ⊙ HasSymm.symm
 
   end IsIsomorphismRelation
 
@@ -430,11 +428,11 @@ end Morphisms
 
 section Functors
 
-  variable {α : Sort u} {V : Sort v} [IsKind V] [HasInstanceArrows V]
+  variable {α : Sort u} {U : Universe} [HasFunOp U] [hasArrows : HasFunctorialArrows U]
 
   namespace idFun
 
-    variable (R : GeneralizedRelation α V)
+    variable (R : GeneralizedRelation α U)
 
     instance isReflFunctor  [HasRefl  R] : IsReflFunctor  R R (HasFunOp.idFun' _) :=
     ⟨λ a   => HasRefl.refl (ident R a)⟩
@@ -452,20 +450,18 @@ section Functors
 
   namespace constFun
 
-    variable (R : GeneralizedRelation α V) {β : V} (c : β)
+    variable (R : GeneralizedRelation α U) {β : U} (c : β)
 
-    def idArrow := (HasInstanceArrows.instArrows V β).isPreorder.refl c
+    def idArrow : c ⇝ c := ident (hasArrows.Arrow β) c
 
     instance isReflFunctor  [HasRefl  R] : IsReflFunctor  R (ConstRel α c) (HasFunOp.constFun' _ c) :=
     ⟨λ _   => idArrow c⟩
 
     instance isSymmFunctor  [HasSymm  R] : IsSymmFunctor  R (ConstRel α c) (HasFunOp.constFun' _ c) :=
-    ⟨λ _   => Eq.ndrec (motive := λ b => HasInstances.Inst (HasInstanceArrows.InstArrow V β c b))
-                       (idArrow c) (Eq.symm (ConstRel.symmEq  α c))⟩
+    ⟨λ _   => Eq.ndrec (motive := λ b : β => ⌈c ⇝ b⌉) (idArrow c) (Eq.symm (ConstRel.symmEq  α c))⟩
 
     instance isTransFunctor [HasTrans R] : IsTransFunctor R (ConstRel α c) (HasFunOp.constFun' _ c) :=
-    ⟨λ _ _ => Eq.ndrec (motive := λ b => HasInstances.Inst (HasInstanceArrows.InstArrow V β c b))
-                       (idArrow c) (Eq.symm (ConstRel.transEq α c))⟩
+    ⟨λ _ _ => Eq.ndrec (motive := λ b : β => ⌈c ⇝ b⌉) (idArrow c) (Eq.symm (ConstRel.transEq α c))⟩
 
     instance isPreorderFunctor    [IsPreorder    R] : IsPreorderFunctor    R (ConstRel α c) (HasFunOp.constFun' _ c) := ⟨⟩
     instance isEquivalenceFunctor [IsEquivalence R] : IsEquivalenceFunctor R (ConstRel α c) (HasFunOp.constFun' _ c) := ⟨⟩
@@ -474,23 +470,23 @@ section Functors
 
   namespace compFun
 
-    variable {R S T : GeneralizedRelation α V} (F : BaseFunctor R S) (G : BaseFunctor S T)
+    variable {R S T : GeneralizedRelation α U} (F : BaseFunctor R S) (G : BaseFunctor S T)
 
     instance isReflFunctor  [HasRefl  R] [HasRefl  S] [HasRefl  T] [hF : IsReflFunctor  R S F] [hG : IsReflFunctor  S T G] :
       IsReflFunctor  R T (G ⊙' F) :=
-    ⟨λ a   => let e₁ : G (F (ident R a)) ⇝ G (ident S a) := HasInstanceArrows.arrCongrArg' V G (hF.respectsRefl a);
+    ⟨λ a   => let e₁ : G (F (ident R a)) ⇝ G (ident S a) := HasFunctorialArrows.arrowCongrArg' U G (hF.respectsRefl a);
               let e₂ : G (ident S a) ⇝ ident T a         := hG.respectsRefl a;
               HasTrans.trans' e₁ e₂⟩
 
     instance isSymmFunctor  [HasSymm  R] [HasSymm  S] [HasSymm  T] [hF : IsSymmFunctor  R S F] [hG : IsSymmFunctor  S T G] :
       IsSymmFunctor  R T (G ⊙' F) :=
-    ⟨λ f   => let e₁ : G (F f⁻¹) ⇝ G (F f)⁻¹   := HasInstanceArrows.arrCongrArg' V G (hF.respectsSymm f);
+    ⟨λ f   => let e₁ : G (F f⁻¹) ⇝ G (F f)⁻¹   := HasFunctorialArrows.arrowCongrArg' U G (hF.respectsSymm f);
               let e₂ : G (F f)⁻¹ ⇝ (G (F f))⁻¹ := hG.respectsSymm (F f);
               HasTrans.trans' e₁ e₂⟩
 
     instance isTransFunctor [HasTrans R] [HasTrans S] [HasTrans T] [hF : IsTransFunctor R S F] [hG : IsTransFunctor S T G] :
       IsTransFunctor R T (G ⊙' F) :=
-    ⟨λ f g => let e₁ : G (F (g • f)) ⇝ G (F g • F f)     := HasInstanceArrows.arrCongrArg' V G (hF.respectsTrans f g);
+    ⟨λ f g => let e₁ : G (F (g • f)) ⇝ G (F g • F f)     := HasFunctorialArrows.arrowCongrArg' U G (hF.respectsTrans f g);
               let e₂ : G (F g • F f) ⇝ G (F g) • G (F f) := hG.respectsTrans (F f) (F g);
               HasTrans.trans' e₁ e₂⟩
 
@@ -501,35 +497,39 @@ section Functors
 
   end compFun
 
+  -- TODO: HasIdFun etc.
+
 end Functors
 
 
 
 section NaturalTransformations
 
-  variable {α : Sort u} {V : Sort v} {W : Sort w} [IsKind V] [IsKind W] [HasInstanceEquivalences W] [HasIsFun V W]
+  variable {α : Sort u} {V W : Universe} [HasInternalFunctors W] [HasFunctorialEquivalences W] [HasExternalFunctors V W]
            {β : Sort w} (R : GeneralizedRelation α V) (S : GeneralizedRelation β W)
+
+  instance : HasFunctorialArrows W := HasFunctorialEquivalences.toHasFunctorialArrows W
 
   namespace IsNaturalTransformation
 
-    def refl  [h : IsMorphismRelation    S] {mF       : α → β}
+    def refl  [IsPreorder    S] [h : IsMorphismRelation    S] {mF       : α → β}
               (F : ∀ {a b}, R a b ⟶' S (mF a) (mF b)) :
-      IsNaturalTransformation R S F F (λ a => h.refl (mF a)) :=
+      IsNatural R S F F (λ a => ident S (mF a)) :=
     ⟨λ f => HasTrans.trans' (h.rightId (F f)) (HasSymm.symm' (h.leftId (F f)))⟩
 
-    def symm  [h : IsIsomorphismRelation S] {mF mG    : α → β}
+    def symm  [IsEquivalence S] [h : IsIsomorphismRelation S] {mF mG    : α → β}
               (F : ∀ {a b}, R a b ⟶' S (mF a) (mF b)) (G : ∀ {a b}, R a b ⟶' S (mG a) (mG b))
-              (n : ∀ a, S (mF a) (mG a)) [hn : IsNaturalTransformation R S F G n] :
-      IsNaturalTransformation R S G F (λ a => h.symm (n a)) :=
-    ⟨λ {a b} f => HasSymm.symm' ((IsIsomorphismRelation.leftRightMul W (n a) (F f) (G f) (n b)).mpr (hn.nat f))⟩
+              (n : ∀ a, S (mF a) (mG a)) [hn : IsNatural R S F G n] :
+      IsNatural R S G F (λ a => (n a)⁻¹) :=
+    ⟨λ {a b} f => HasSymm.symm' ((IsIsomorphismRelation.leftRightMul (n a) (F f) (G f) (n b)).mpr (hn.nat f))⟩
 
-    def trans [h : IsCompositionRelation S] {mF mG mH : α → β}
+    def trans [HasTrans      S] [h : IsCompositionRelation S] {mF mG mH : α → β}
               (F : ∀ {a b}, R a b ⟶' S (mF a) (mF b)) (G : ∀ {a b}, R a b ⟶' S (mG a) (mG b)) (H : ∀ {a b}, R a b ⟶' S (mH a) (mH b))
-              (nFG : ∀ a, S (mF a) (mG a))                 (nGH : ∀ a, S (mG a) (mH a))
-              [hnFG : IsNaturalTransformation R S F G nFG] [hnGH : IsNaturalTransformation R S G H nGH] :
-      IsNaturalTransformation R S F H (λ a => h.trans (nFG a) (nGH a)) :=
-    ⟨λ {a b} f => let e₁ := IsCompositionRelation.applyAssocLR_left W (IsCompositionRelation.comp_congrArg_left  W (f := nFG a) (hnGH.nat f));
-                  let e₂ := IsCompositionRelation.applyAssocRL      W (IsCompositionRelation.comp_congrArg_right W (g := nGH b) (hnFG.nat f));
+              (nFG : ∀ a, S (mF a) (mG a))   (nGH : ∀ a, S (mG a) (mH a))
+              [hnFG : IsNatural R S F G nFG] [hnGH : IsNatural R S G H nGH] :
+      IsNatural R S F H (λ a => nGH a • nFG a) :=
+    ⟨λ {a b} f => let e₁ := IsCompositionRelation.applyAssocLR_left⟮IsCompositionRelation.comp_congrArg_left  (f := nFG a) (hnGH.nat f)⟯;
+                  let e₂ := IsCompositionRelation.applyAssocRL     ⟮IsCompositionRelation.comp_congrArg_right (g := nGH b) (hnFG.nat f)⟯;
                   HasTrans.trans' e₁ e₂⟩
 
   end IsNaturalTransformation
