Structure/Generic/Categories.lean
@@ -1,0 +1,60 @@
+--  An abstract formalization of "isomorphism is equality up to relabeling"
+-- -------------------------------------------------------------------------
+--
+-- See `README.md` for more info.
+--
+-- This file contains definitions of (potentially higher) categories and groupoids.
+
+
+
+import Structure.Generic.Axioms
+import Structure.Generic.Functors
+
+
+
+section Categories
+
+  variable (M : Universe) [HasInternalFunctors M] [HasInstanceArrows M] (α : Sort u)
+
+  class IsCategory extends HasArrows α M where
+  [isMor : IsMorphismRelation Arrow]
+
+  namespace IsCategory
+
+    variable [h : IsCategory M α]
+
+    instance hasMor : IsMorphismRelation h.Arrow := h.isMor
+
+  end IsCategory
+
+  class IsGroupoid extends HasEquivalences α M where
+  [isIso : IsIsomorphismRelation Equiv]
+
+  namespace IsGroupoid
+
+    variable [h : IsGroupoid M α]
+
+    instance hasIso : IsIsomorphismRelation h.Equiv := h.isIso
+
+  end IsGroupoid
+
+end Categories
+
+
+
+section BundledCategories
+
+  variable (M : Universe) [HasInternalFunctors M] [HasInstanceArrows M]
+
+  @[reducible] def Category := Bundled (IsCategory M)
+  @[reducible] def Groupoid := Bundled (IsGroupoid M)
+
+end BundledCategories
+
+
+
+-- TODO: Show that:
+-- * the universes of categories and groupoids have nice properties
+--   (-> bundled functors -> natural transformation as equivalence -> internal functors), and
+-- * universes with certain properties are actually categories/groupoids
+--   (-> category of categories, groupoid of groupoids).
