Structure/Generic/Instances.lean
@@ -15,62 +15,60 @@ import mathlib4_experiments.Data.Equiv.Basic
 
 
 set_option autoBoundImplicitLocal false
+set_option pp.universes true
 
-universes u v u' v' w
+universes u uu v vv w
 
 
 
-namespace AnySort
+namespace SortUniverse
 
-  instance hasInstances : HasInstances (Sort u) := ⟨id⟩
+  instance hasExternalFunctors : HasExternalFunctors sortUniverse.{u} sortUniverse.{v} := ⟨λ _ => True⟩
 
-  instance hasIsFun : HasIsFun (Sort u) (Sort v) := ⟨λ _ => True⟩
-
-  instance hasFun : HasFun (Sort u) :=
+  instance hasInternalFunctors : HasInternalFunctors sortUniverse.{u} :=
   { Fun      := λ α β => α → β,
     funEquiv := λ α β => { toFun    := λ f      => ⟨f, trivial⟩,
                            invFun   := λ F      => F.f,
                            leftInv  := λ f      => rfl,
                            rightInv := λ ⟨f, _⟩ => rfl } }
 
-  instance hasFunOp : HasFunOp (Sort u) :=
-  { idIsFun         := λ _     => trivial,
-    constIsFun      := λ _ _ _ => trivial,
-    constFunIsFun   := λ _ _   => trivial,
+  instance hasIdFun    : HasIdFun    sortUniverse.{u}                                   := ⟨λ _     => trivial⟩
+  instance hasConstFun : HasConstFun sortUniverse.{u} sortUniverse.{v}                  := ⟨λ _ _ _ => trivial⟩
+  instance hasCompFun  : HasCompFun  sortUniverse.{u} sortUniverse.{v} sortUniverse.{w} := ⟨λ _ _   => trivial⟩
+
+  instance hasFunOp : HasFunOp sortUniverse.{u} :=
+  { constFunIsFun   := λ _ _   => trivial,
     appIsFun        := λ _ _   => trivial,
     appFunIsFun     := λ _ _   => trivial,
     dupIsFun        := λ _     => trivial,
     dupFunIsFun     := λ _ _   => trivial,
-    compIsFun       := λ _ _   => trivial,
     compFunIsFun    := λ _ _   => trivial,
     compFunFunIsFun := λ _ _ _ => trivial }
 
-  instance isKind : IsKind (Sort u) := ⟨⟩
-
-end AnySort
+end SortUniverse
 
 
 
-def UnivRel (α : Sort u) : α → α → Prop := λ _ _ => True
+def UnivRel (α : Sort u) : GeneralizedRelation α propUniverse := λ _ _ => True
 
 def UnivRel.isEquivalence {α : Sort u} : Equivalence (UnivRel α) :=
 ⟨λ _ => trivial, λ _ => trivial, λ _ _ => trivial⟩
 
-def EquivRel : GeneralizedRelation (Type u) (Type u) := Equiv
+def EquivRel : GeneralizedRelation (Type u) typeUniverse.{u} := Equiv
 
 namespace GeneralizedRelation.IsEquivalence
 
   -- Every equivalence relation can trivially be converted to an instance of `IsEquivalence`.
-  instance relEquiv {α : Sort u} {r : α → α → Prop} (e : Equivalence r) : IsEquivalence r :=
+  instance relEquiv {α : Sort u} {R : GeneralizedRelation α propUniverse} (e : Equivalence R) : IsEquivalence R :=
   { refl  := e.refl,
     symm  := e.symm,
     trans := e.trans }
 
   -- So these are the instances that we obtain directly from Lean.
-  instance univ   (α : Sort u)                : IsEquivalence (UnivRel α) := relEquiv UnivRel.isEquivalence
-  instance iff                                : IsEquivalence Iff         := relEquiv Iff.isEquivalence
-  instance eq     (α : Sort u)                : IsEquivalence (@Eq α)     := relEquiv Eq.isEquivalence
-  instance setoid (α : Sort u) [s : Setoid α] : IsEquivalence s.r         := relEquiv s.iseqv
+  instance univ   (α : Sort u)                : IsEquivalence (V := propUniverse) (UnivRel α) := relEquiv UnivRel.isEquivalence
+  instance iff                                : IsEquivalence (V := propUniverse) Iff         := relEquiv Iff.isEquivalence
+  instance eq     (α : Sort u)                : IsEquivalence (V := propUniverse) (@Eq α)     := relEquiv Eq.isEquivalence
+  instance setoid (α : Sort u) [s : Setoid α] : IsEquivalence (V := propUniverse) s.r         := relEquiv s.iseqv
 
   instance equiv : IsEquivalence EquivRel :=
   { refl  := Equiv.refl,
@@ -81,23 +79,25 @@ end GeneralizedRelation.IsEquivalence
 
 
 
+-- TODO: Convert products, `Iff`, and `Equiv` to general axioms and an instance similar to `Fun` -> `Arrow`.
+
 namespace HasProducts
 
-  instance : GeneralizedRelation.HasSymm And := ⟨λ h => ⟨h.right, h.left⟩⟩
-  instance : HasProducts Prop Prop := ⟨And⟩
+  instance : GeneralizedRelation.HasSymm (V := propUniverse) And := ⟨λ h => ⟨h.right, h.left⟩⟩
+  instance : HasProducts Prop propUniverse := ⟨And⟩
 
-  instance : GeneralizedRelation.HasSymm Prod := ⟨λ p => ⟨p.snd, p.fst⟩⟩
-  instance : HasProducts (Type u) (Type u) := ⟨Prod⟩
+  instance : GeneralizedRelation.HasSymm (V := typeUniverse.{u}) Prod := ⟨λ p => ⟨p.snd, p.fst⟩⟩
+  instance : HasProducts (Type u) typeUniverse.{u} := ⟨Prod⟩
 
 end HasProducts
 
 namespace HasEquivalences
 
-  def univ   (α : Sort u)                : HasEquivalences α        Prop     := ⟨UnivRel α⟩
-  instance iff                           : HasEquivalences Prop     Prop     := ⟨Iff⟩
-  def eq     (α : Sort u)                : HasEquivalences α        Prop     := ⟨Eq⟩
-  def setoid (α : Sort u) [s : Setoid α] : HasEquivalences α        Prop     := ⟨s.r⟩
-  instance equiv                         : HasEquivalences (Type u) (Type u) := ⟨EquivRel⟩
+  def univ   (α : Sort u)                : HasEquivalences α        propUniverse     := ⟨UnivRel α⟩
+  instance iff                           : HasEquivalences Prop     propUniverse     := ⟨Iff⟩
+  def eq     (α : Sort u)                : HasEquivalences α        propUniverse     := ⟨Eq⟩
+  def setoid (α : Sort u) [s : Setoid α] : HasEquivalences α        propUniverse     := ⟨s.r⟩
+  instance equiv                         : HasEquivalences (Type u) typeUniverse.{u} := ⟨EquivRel⟩
 
 end HasEquivalences
 
@@ -107,46 +107,50 @@ namespace HasInstanceEquivalences
 
   -- By specializing here, we avoid invoking proof irrelevance explicitly.
   -- Instead, we just declare all proofs to be equivalent according to our own notion of equivalence.
-  instance prop : HasInstanceEquivalences' Prop :=
-  { EquivKind       := Prop,
-    equivIsKind     := AnySort.isKind,
-    hasEquivalences := HasEquivalences.univ,
-    equivCongr      := λ _ _ => trivial }
+  instance prop       : HasInstanceEquivalences propUniverse     := ⟨propUniverse, UnivRel⟩
+  instance typeWithEq : HasInstanceEquivalences typeUniverse.{u} := ⟨propUniverse, @Eq⟩
 
-  instance typeWithEq : HasInstanceEquivalences' (Type u) :=
-  { EquivKind       := Prop,
-    equivIsKind     := AnySort.isKind,
-    hasEquivalences := HasEquivalences.eq,
-    equivCongr      := congr }
+  instance : HasInstanceArrows propUniverse     := HasInstanceEquivalences.toHasInstanceArrows propUniverse
+  instance : HasInstanceArrows typeUniverse.{u} := HasInstanceEquivalences.toHasInstanceArrows typeUniverse.{u}
 
 end HasInstanceEquivalences
+
+namespace HasFunctorialEquivalences
+  
+  instance prop       : HasFunctorialEquivalences propUniverse :=
+  { equivCongr := λ _ _ => trivial }
+
+  instance typeWithEq : HasFunctorialEquivalences typeUniverse.{u} :=
+  { equivCongr := congr }
+
+end HasFunctorialEquivalences
 
 
 
 namespace PropRel
 
-  variable {α : Sort u} (r : α → α → Prop) [GeneralizedRelation.IsEquivalence r]
+  variable {α : Sort u} (R : GeneralizedRelation α propUniverse) [GeneralizedRelation.IsEquivalence R]
 
-  instance isCompositionRelation : IsCompositionRelation r :=
+  instance isCompositionRelation : IsCompositionRelation R :=
   { assocLR := λ _ _ _ => trivial,
     assocRL := λ _ _ _ => trivial }
 
-  instance isMorphismRelation : IsMorphismRelation r :=
+  instance isMorphismRelation : IsMorphismRelation R :=
   { leftId  := λ _ => trivial,
     rightId := λ _ => trivial }
 
-  instance isIsomorphismRelation : IsIsomorphismRelation r :=
+  instance isIsomorphismRelation : IsIsomorphismRelation R :=
   { leftInv  := λ _   => trivial,
     rightInv := λ _   => trivial,
     invInv   := λ _   => trivial,
     compInv  := λ _ _ => trivial,
     idInv    := λ _   => trivial }
 
-  variable (s : α → α → Prop) [GeneralizedRelation.IsEquivalence s] (F : BaseFunctor r s)
+  variable (S : GeneralizedRelation α propUniverse) [GeneralizedRelation.IsEquivalence S] (F : BaseFunctor R S)
 
-  instance isReflFunctor  : IsReflFunctor  r s F := ⟨λ _   => trivial⟩
-  instance isSymmFunctor  : IsSymmFunctor  r s F := ⟨λ _   => trivial⟩
-  instance isTransFunctor : IsTransFunctor r s F := ⟨λ _ _ => trivial⟩
+  instance isReflFunctor  : IsReflFunctor  R S F := ⟨λ _   => trivial⟩
+  instance isSymmFunctor  : IsSymmFunctor  R S F := ⟨λ _   => trivial⟩
+  instance isTransFunctor : IsTransFunctor R S F := ⟨λ _ _ => trivial⟩
 
 end PropRel
 
@@ -171,51 +175,53 @@ end EquivRel
 
 
 
-def TypeClass := Sort u → Sort v
-
-structure Bundled (C : TypeClass.{u, v}) where
-(α    : Sort u)
-(inst : C α)
-
 namespace Bundled
 
-  instance hasInstances (C : TypeClass) : HasInstances (Bundled C) := ⟨Bundled.α⟩
+  class HasFunctoriality (C : TypeClass.{u, u + 1, uu} (Sort u)) (D : TypeClass.{v, v + 1, vv} (Sort v)) where
+  (IsFunctorial {S : Bundled C} {T : Bundled D} : (S → T) → Sort w)
 
-  class HasFunctoriality (C D : TypeClass) where
-  (IsFunctorial {S : Bundled.{u, v} C} {T : Bundled.{u', v'} D} : (S → T) → Sort w)
+  def bundledUniverse (C : TypeClass.{u, u + 1, uu} (Sort u)) : Universe.{u, max (u + 1) uu} := ⟨Bundled C⟩
 
-  instance hasIsFun (C D : TypeClass) [h : HasFunctoriality C D] : HasIsFun (Bundled.{u, v} C) (Bundled.{u', v'} D) := ⟨h.IsFunctorial⟩
+  instance hasExternalFunctors (C : TypeClass.{u, u + 1, uu} (Sort u)) (D : TypeClass.{v, v + 1, vv} (Sort v))
+                               [h : HasFunctoriality C D] :
+    HasExternalFunctors (bundledUniverse.{u, uu} C) (bundledUniverse.{v, vv} D) :=
+  ⟨h.IsFunctorial⟩
 
-  class HasFunctorInstances (C : TypeClass) [hf : HasFunctoriality.{max 1 u w, v, max 1 u w, v, w} C C] where
-  (funInst (S T : Bundled.{max 1 u w, v} C) : C (S ⟶' T))
+  class HasFunctorInstances (C : TypeClass (Sort (max 1 u v)))
+                            [hf : HasFunctoriality.{max 1 u v, uu, max 1 u v, uu, v} C C] where
+  (funInst (S T : bundledUniverse.{max 1 u v, uu} C) : C (S ⟶' T))
 
-  instance hasFun (C : TypeClass) [hf : HasFunctoriality.{max 1 u w, v, max 1 u w, v, w} C C] [h : HasFunctorInstances.{u, v, w} C] :
-    HasFun (Bundled.{max 1 u w, v} C) :=
-  { Fun      := λ S T => ⟨S ⟶' T, h.funInst S T⟩,
+  instance hasInternalFunctors (C : TypeClass (Sort (max 1 u v)))
+                               [hf : HasFunctoriality.{max 1 u v, uu, max 1 u v, uu, v} C C]
+                               [h : HasFunctorInstances.{u, uu, v} C] :
+    HasInternalFunctors (bundledUniverse.{max 1 u v, uu} C) :=
+  { Fun      := λ S T => { α    := S ⟶' T,
+                           inst := h.funInst S T },
     funEquiv := λ S T => Equiv.refl (S ⟶' T) }
 
 end Bundled
 
 
 
-@[reducible] def BundledSetoid : Type (u + 1) := Bundled.{u + 1, u + 1} Setoid
+@[reducible] def bundledSetoid : Universe.{u + 1} := Bundled.bundledUniverse.{u + 1, u + 1} Setoid
 
 namespace BundledSetoid
 
-  instance isSetoid (S : BundledSetoid) : Setoid (HasInstances.Inst S) := S.inst
+  instance isSetoid (S : bundledSetoid) : Setoid ⌈S⌉ := S.inst
+  instance (S : bundledSetoid) : Setoid ⌈S⌉ := isSetoid S
 
-  class IsFunctorial {S T : BundledSetoid} (f : S → T) where
+  class IsFunctorial {S T : bundledSetoid} (f : S → T) where
   (mapEquiv {a b : S} : a ≈ b → f a ≈ f b)
 
-  instance hasFunctoriality : Bundled.HasFunctoriality.{u + 1, u + 1, u' + 1, u' + 1, 1} Setoid Setoid := ⟨IsFunctorial⟩
+  instance hasFunctoriality : Bundled.HasFunctoriality.{u + 1, u + 1, v + 1, v + 1, 1} Setoid Setoid := ⟨IsFunctorial⟩
 
   namespace BundledFunctor
 
-    def Equiv {S T : BundledSetoid} (F G : S ⟶' T) := ∀ a, F a ≈ G a
+    def Equiv {S T : bundledSetoid} (F G : S ⟶' T) := ∀ a, F a ≈ G a
 
     namespace Equiv
 
-      variable {S T : BundledSetoid}
+      variable {S T : bundledSetoid}
 
       theorem refl  (F     : S ⟶' T)                                 : Equiv F F := λ a => Setoid.refl  (F a)
       theorem symm  {F G   : S ⟶' T} (h : Equiv F G)                 : Equiv G F := λ a => Setoid.symm  (h a)
@@ -225,78 +231,37 @@ namespace BundledSetoid
 
     end Equiv
 
-    instance isSetoid (S T : BundledSetoid) : Setoid (S ⟶' T) := ⟨Equiv, Equiv.isEquivalence⟩
+    instance isSetoid (S T : bundledSetoid) : Setoid (S ⟶' T) := ⟨Equiv, Equiv.isEquivalence⟩
     instance hasFunctorInstances : Bundled.HasFunctorInstances.{u + 1, u + 1, 1} Setoid := ⟨isSetoid⟩
 
   end BundledFunctor
 
-  instance hasFun : HasFun BundledSetoid := Bundled.hasFun Setoid
+  instance hasInternalFunctors : HasInternalFunctors bundledSetoid := Bundled.hasInternalFunctors Setoid
 
-  instance hasFunOp : HasFunOp BundledSetoid :=
-  { idIsFun         := λ S           => ⟨λ ha         => ha⟩,
-    constIsFun      := λ S {T} c     => ⟨λ ha         => Setoid.refl c⟩,
-    constFunIsFun   := λ S T         => ⟨λ hc a       => hc⟩,
+  instance hasIdFun    : HasIdFun    bundledSetoid.{u}                                     :=
+  ⟨λ S           => ⟨id⟩⟩
+  instance hasConstFun : HasConstFun bundledSetoid.{u} bundledSetoid.{v}                   :=
+  ⟨λ S {T}   c   => ⟨Function.const _ (Setoid.refl c)⟩⟩
+  instance hasCompFun  : HasCompFun  bundledSetoid.{u} bundledSetoid.{v} bundledSetoid.{w} :=
+  ⟨λ {S T U} F G => ⟨G.isFun.mapEquiv ∘ F.isFun.mapEquiv⟩⟩
+
+  instance hasFunOp : HasFunOp bundledSetoid :=
+  { constFunIsFun   := λ S T         => ⟨λ hc a       => hc⟩,
     appIsFun        := λ {S} a T     => ⟨λ hF         => hF a⟩,
     appFunIsFun     := λ S T         => ⟨λ ha F       => F.isFun.mapEquiv ha⟩,
     dupIsFun        := λ {S T} F     => ⟨λ {a₁ a₂} ha => Setoid.trans (F.isFun.mapEquiv ha a₁) ((F a₂).isFun.mapEquiv ha)⟩,
     dupFunIsFun     := λ S T         => ⟨λ hF a       => hF a a⟩,
-    compIsFun       := λ {S T U} F G => ⟨λ ha         => G.isFun.mapEquiv (F.isFun.mapEquiv ha)⟩,
     compFunIsFun    := λ {S T} F U   => ⟨λ hG a       => hG (F a)⟩,
     compFunFunIsFun := λ S T U       => ⟨λ hF G a     => G.isFun.mapEquiv (hF a)⟩ }
 
-  instance isKind : IsKind BundledSetoid := ⟨⟩
+  instance hasInstanceEquivalences : HasInstanceEquivalences bundledSetoid :=
+  ⟨propUniverse, λ S => (isSetoid S).r⟩
 
-  instance hasInstanceEquivalences : HasInstanceEquivalences' BundledSetoid :=
-  { EquivKind       := Prop,
-    equivIsKind     := AnySort.isKind,
-    hasEquivalences := λ S => HasEquivalences.setoid (HasInstances.Inst S),
-    equivCongr      := λ {S T F G a b} h₁ h₂ => Setoid.trans (h₁ a) (G.isFun.mapEquiv h₂) }
+  instance hasFunctorialEquivalences : HasFunctorialEquivalences bundledSetoid :=
+  { equivCongr := λ {S T F G a b} h₁ h₂ => Setoid.trans (h₁ a) (G.isFun.mapEquiv h₂) }
 
-  def eq (α : Sort u) : Bundled Setoid :=
+  def eq (α : Type u) : bundledSetoid :=
   { α    := α,
     inst := ⟨Eq, Eq.isEquivalence⟩ }
 
 end BundledSetoid
-
-
-
--- TODO: Where exactly does this fit into the axioms?
--- It is an equivalence between instances of IsKind, with a dependent equivalence given by `e a = b`...
-
-class IsFunctorialTypeClass (C : TypeClass) where
-(mapEquiv      {α β   : Sort u}                         : α ≃ β → C α ≃ C β)
-(respectsRefl  (α     : Sort u)                         : mapEquiv (Equiv.refl  α)   = Equiv.refl  (C α))
-(respectsSymm  {α β   : Sort u} (e : α ≃ β)             : mapEquiv (Equiv.symm  e)   = Equiv.symm  (mapEquiv e))
-(respectsTrans {α β γ : Sort u} (e : α ≃ β) (f : β ≃ γ) : mapEquiv (Equiv.trans e f) = Equiv.trans (mapEquiv e) (mapEquiv f))
-
-structure TypeFunctor where
-(C     : TypeClass)
-[isFun : IsFunctorialTypeClass C]
-
-namespace TypeFunctor
-
-  -- TODO: This duplicates generic proofs.
-
-  instance (F : TypeFunctor) : IsFunctorialTypeClass F.C := F.isFun
-
-  instance : IsFunctorialTypeClass id :=
-  { mapEquiv      := id,
-    respectsRefl  := λ _   => rfl,
-    respectsSymm  := λ _   => rfl,
-    respectsTrans := λ _ _ => rfl }
-
-  def funId : TypeFunctor := ⟨id⟩
-
-  instance (C D : TypeClass) [hC : IsFunctorialTypeClass C] [hD : IsFunctorialTypeClass D] :
-    IsFunctorialTypeClass (D ∘ C) :=
-  { mapEquiv      := hD.mapEquiv ∘ hC.mapEquiv,
-    respectsRefl  := λ α   => Eq.trans (congrArg hD.mapEquiv (hC.respectsRefl  α))
-                                       (hD.respectsRefl (C α)),
-    respectsSymm  := λ e   => Eq.trans (congrArg hD.mapEquiv (hC.respectsSymm  e))
-                                       (hD.respectsSymm (hC.mapEquiv e)),
-    respectsTrans := λ e f => Eq.trans (congrArg hD.mapEquiv (hC.respectsTrans e f))
-                                       (hD.respectsTrans (hC.mapEquiv e) (hC.mapEquiv f)) }
-
-  def funComp (F G : TypeFunctor) : TypeFunctor := ⟨G.C ∘ F.C⟩
-
-end TypeFunctor
