Structure/Generic/Mapped.lean
@@ -15,11 +15,11 @@ open GeneralizedRelation
 
 set_option autoBoundImplicitLocal false
 
-universes u v w w'
+universes u v w
 
 
 
-def mapOperation {α : Sort u} {β : Sort v} {ω : Sort w} (m : ω → α) (op : α → α → β) :
+def mapOperation {α : Sort u} {β : Sort v} (op : α → α → β) {ω : Sort w} (m : ω → α) :
   ω → ω → β :=
 λ a b => op (m a) (m b)
 
@@ -27,9 +27,8 @@ def mapOperation {α : Sort u} {β : Sort v} {ω : Sort w} (m : ω → α) (op :
 
 namespace GeneralizedProperty
 
-  variable {α : Sort u} {V : Sort v} [HasInstances V]
+  variable {α : Sort u} {V : Universe} (P : GeneralizedProperty α V)
            {ω : Sort w} (m : ω → α)
-           (P : GeneralizedProperty α V)
 
   instance mapInst [h : HasInst P] : HasInst (P ∘ m) := ⟨λ a => h.inst (m a)⟩
 
@@ -39,15 +38,18 @@ end GeneralizedProperty
 
 namespace GeneralizedRelation
 
-  variable {α : Sort u} {V : Sort v} [IsKind V]
-           {ω : Sort w} (m : ω → α) (R : GeneralizedRelation α V)
+  variable {α : Sort u} {V : Universe} (R : GeneralizedRelation α V)
+           {ω : Sort w} (m : ω → α)
 
-  instance mapRefl  [h : HasRefl  R] : HasRefl  (mapOperation m R) := ⟨λ a => h.refl (m a)⟩
-  instance mapSymm  [h : HasSymm  R] : HasSymm  (mapOperation m R) := ⟨h.symm⟩
-  instance mapTrans [h : HasTrans R] : HasTrans (mapOperation m R) := ⟨h.trans⟩
+  instance mapRefl  [h : HasRefl  R] : HasRefl  (mapOperation R m) := ⟨λ a => h.refl (m a)⟩
 
-  instance mapPreorder    [IsPreorder    R] : IsPreorder    (mapOperation m R) := ⟨⟩
-  instance mapEquivalence [IsEquivalence R] : IsEquivalence (mapOperation m R) := ⟨⟩
+  variable [HasInternalFunctors V]
+
+  instance mapSymm  [h : HasSymm  R] : HasSymm  (mapOperation R m) := ⟨h.symm⟩
+  instance mapTrans [h : HasTrans R] : HasTrans (mapOperation R m) := ⟨h.trans⟩
+
+  instance mapPreorder    [IsPreorder    R] : IsPreorder    (mapOperation R m) := ⟨⟩
+  instance mapEquivalence [IsEquivalence R] : IsEquivalence (mapOperation R m) := ⟨⟩
 
 end GeneralizedRelation
 
@@ -55,22 +57,22 @@ end GeneralizedRelation
 
 section Morphisms
 
-  variable {α : Sort u} {V : Sort v} [IsKind V] [HasInstanceArrows V]
-           {ω : Sort w} (m : ω → α)
+  variable {α : Sort u} {V : Universe} [HasInternalFunctors V] [HasInstanceArrows V]
            (R : GeneralizedRelation α V)
+           {ω : Sort w} (m : ω → α)
 
-  instance mapComposition  [h : IsCompositionRelation  R] :
-    IsCompositionRelation (mapOperation m R) :=
+  instance mapComposition  [HasTrans      R] [h : IsCompositionRelation R] :
+    IsCompositionRelation (mapOperation R m) :=
   { assocLR  := h.assocLR,
     assocRL  := h.assocRL }
 
-  instance mapMorphisms    [h : IsMorphismRelation    R] :
-    IsMorphismRelation    (mapOperation m R) :=
+  instance mapMorphisms    [IsPreorder    R] [h : IsMorphismRelation    R] :
+    IsMorphismRelation    (mapOperation R m) :=
   { leftId   := h.leftId,
     rightId  := h.rightId }
 
-  instance mapIsomorphisms [h : IsIsomorphismRelation R] :
-    IsIsomorphismRelation (mapOperation m R) :=
+  instance mapIsomorphisms [IsEquivalence R] [h : IsIsomorphismRelation R] :
+    IsIsomorphismRelation (mapOperation R m) :=
   { leftInv  := h.leftInv,
     rightInv := h.rightInv,
     invInv   := h.invInv,
@@ -83,27 +85,29 @@ end Morphisms
 
 section Functors
 
-  variable {α : Sort u} {V : Sort v} {W : Sort w} [IsKind V] [IsKind W] [HasInstanceArrows W] [HasIsFun V W]
-           {ω : Sort w'} (m : ω → α)
+  variable {α : Sort u} {V W : Universe} [HasInstanceArrows W] [HasExternalFunctors V W]
            (R : GeneralizedRelation α V) (S : GeneralizedRelation α W)
            (F : BaseFunctor R S)
+           {ω : Sort w} (m : ω → α)
 
   instance mapReflFunctor  [HasRefl  R] [HasRefl  S] [h : IsReflFunctor  R S F] :
-    IsReflFunctor  (mapOperation m R) (mapOperation m S) F :=
+    IsReflFunctor  (mapOperation R m) (mapOperation S m) F :=
   ⟨λ a => h.respectsRefl (m a)⟩
 
+  variable [HasInternalFunctors V] [HasInternalFunctors W]
+
   instance mapSymmFunctor  [HasSymm  R] [HasSymm S ] [h : IsSymmFunctor  R S F] :
-    IsSymmFunctor  (mapOperation m R) (mapOperation m S) F :=
+    IsSymmFunctor  (mapOperation R m) (mapOperation S m) F :=
   ⟨h.respectsSymm⟩
 
   instance mapTransFunctor [HasTrans R] [HasTrans S] [h : IsTransFunctor R S F] :
-    IsTransFunctor (mapOperation m R) (mapOperation m S) F :=
+    IsTransFunctor (mapOperation R m) (mapOperation S m) F :=
   ⟨h.respectsTrans⟩
 
   instance mapPreorderFunctor    [IsPreorder    R] [IsPreorder    S] [IsPreorderFunctor    R S F] :
-    IsPreorderFunctor    (mapOperation m R) (mapOperation m S) F := ⟨⟩
+    IsPreorderFunctor    (mapOperation R m) (mapOperation S m) F := ⟨⟩
   instance mapEquivalenceFunctor [IsEquivalence R] [IsEquivalence S] [IsEquivalenceFunctor R S F] :
-    IsEquivalenceFunctor (mapOperation m R) (mapOperation m S) F := ⟨⟩
+    IsEquivalenceFunctor (mapOperation R m) (mapOperation S m) F := ⟨⟩
 
 end Functors
 
@@ -111,14 +115,14 @@ end Functors
 
 section NaturalTransformations
 
-  variable {α : Sort u} {β : Sort w} {V : Sort v} {W : Sort w} [IsKind V] [IsKind W] [HasInstanceEquivalences W] [HasIsFun V W]
-           {ω : Sort w'} (m : ω → α)
-           (R : GeneralizedRelation α V) (S : GeneralizedRelation β W) [HasTrans S]
+  variable {α : Sort u} {β : Sort v} {V W : Universe} [HasInternalFunctors W] [HasInstanceEquivalences W] [HasExternalFunctors V W]
+           (R : GeneralizedRelation α V) (S : GeneralizedRelation β W) [h : HasTrans S]
            {mF mG : α → β} (F : ∀ {a b}, R a b ⟶' S (mF a) (mF b)) (G : ∀ {a b}, R a b ⟶' S (mG a) (mG b))
            (n : ∀ a, S (mF a) (mG a))
+           {ω : Sort w} (m : ω → α)
   
-  instance mapNaturalTransformation [h : IsNaturalTransformation R S F G n] :
-    IsNaturalTransformation (mapOperation m R) S F G (λ a => n (m a)) :=
+  instance mapNaturality [h : IsNatural R S F G n] :
+    IsNatural (mapOperation R m) S F G (λ a => n (m a)) :=
   ⟨h.nat⟩
 
 end NaturalTransformations
